Clean up the theory of bags: * overload various arithmetic operators (+,-,<,<=) (but make these   overload choices appear at the end of the list) * add new syntax for BAG_IN (<:), with a Unicode version too (U+22F2) * remove strange BAG_delta operation that was only ever used in my   PhD, and became incomprehensible to me about the day after I   submitted * tidy up a number of proofs, removing the need for the mnUtils file,   full of "conveniences" from my PhD.

src/bag/bagScript.sml
@@ -1,8 +1,6 @@
-open HolKernel Parse boolLib boolSimps
-     numLib Prim_rec mnUtils pred_setTheory BasicProvers SingleStep
+open HolKernel Parse boolLib boolSimps bossLib
+     numLib Prim_rec pred_setTheory BasicProvers SingleStep
      metisLib dividesTheory arithmeticTheory
-
-val hol_ss = mn_ss;
 
 fun ARITH q = EQT_ELIM (ARITH_CONV (Parse.Term q));
 
@@ -24,7 +22,7 @@ val EMPTY_BAG = new_definition (
 val EMPTY_BAG_alt = store_thm (
   "EMPTY_BAG_alt",
   ``EMPTY_BAG:'a bag = \x.0``,
-  FUN_EQ_TAC THEN SIMP_TAC hol_ss [EMPTY_BAG]);
+  SIMP_TAC std_ss [EMPTY_BAG, FUN_EQ_THM]);
 
 val BAG_INN = new_definition(
   "BAG_INN",
@@ -43,12 +41,21 @@ val BAG_IN = new_definition (
   "BAG_IN",
   ``BAG_IN (e:'a) b = BAG_INN e 1 b``);
 
+val _ = set_fixity "<:" (Infix(NONASSOC, 425))
+val _ = overload_on ("<:", ``BAG_IN``)
+val _ = Unicode.unicode_version {tmnm = "<:", u = UTF8.chr 0x22F2}
+        (* U+22F2 looks like ⋲ in your current font *)
+
 val BAG_UNION = new_definition ("BAG_UNION",
                 ``BAG_UNION b (c:'a bag) = \x. b x + c x``);
+val _ = overload_on ("+", ``BAG_UNION``)
+val _ = send_to_back_overload "+" {Name = "BAG_UNION", Thy = "bag"}
 
 val BAG_DIFF = new_definition (
   "BAG_DIFF",
   ``BAG_DIFF b1 (b2:'a bag) = \x. b1 x - b2 x``);
+val _ = overload_on ("-", ``BAG_DIFF``)
+val _ = send_to_back_overload "-" {Name = "BAG_DIFF", Thy = "bag"}
 
 val BAG_INSERT = new_definition (
   "BAG_INSERT",
@@ -62,13 +69,11 @@ val _ = add_listform {cons = "BAG_INSERT", nilstr = "EMPTY_BAG",
 val BAG_cases = Q.store_thm(
   "BAG_cases",
   `!b. (b = EMPTY_BAG) \/ (?b0 e. b = BAG_INSERT e b0)`,
-  SIMP_TAC hol_ss [EMPTY_BAG, BAG_INSERT] THEN
-  CONV_TAC (DEPTH_CONV FUN_EQ_CONV) THEN
-  SIMP_TAC hol_ss [] THEN GEN_TAC THEN
-  Q.ASM_CASES_TAC `!x. b x = 0` THEN ARWT THEN
-  FULL_SIMP_TAC hol_ss [] THEN MAP_EVERY Q.EXISTS_TAC [
+  SIMP_TAC std_ss [EMPTY_BAG, BAG_INSERT, FUN_EQ_THM] THEN Q.X_GEN_TAC `b` THEN
+  Q.ASM_CASES_TAC `!x. b x = 0` THEN SRW_TAC [][] THEN
+  FULL_SIMP_TAC std_ss [] THEN MAP_EVERY Q.EXISTS_TAC [
     `\y. if (y = x) then b x - 1 else b y`, `x`
-  ] THEN ASM_SIMP_TAC hol_ss [fCOND_OUT_THM, aCOND_OUT_THM]);
+  ] THEN SRW_TAC [ARITH_ss][]);
 
 val BAG_INTER = Q.new_definition(
   "BAG_INTER",
@@ -82,19 +87,20 @@ val _ = print "Properties relating BAG_IN(N) to other functions\n"
 val BAG_INN_0 = store_thm (
   "BAG_INN_0",
   ``!b e:'a. BAG_INN e 0 b``,
-  SIMP_TAC hol_ss [BAG_INN]);
+  SIMP_TAC arith_ss [BAG_INN]);
+val _ = export_rewrites ["BAG_INN_0"]
 
 val BAG_INN_LESS = Q.store_thm(
   "BAG_INN_LESS",
   `!b e n m. BAG_INN e n b /\ m < n ==> BAG_INN e m b`,
-  SIMP_TAC hol_ss [BAG_INN]);
+  SIMP_TAC arith_ss [BAG_INN]);
 
 val BAG_IN_BAG_INSERT = store_thm(
   "BAG_IN_BAG_INSERT",
   ``!b e1 e2:'a.
         BAG_IN e1 (BAG_INSERT e2 b) = (e1 = e2) \/ BAG_IN e1 b``,
-  SIMP_TAC hol_ss [BAG_IN, BAG_INN, BAG_INSERT] THEN
-  REPEAT GEN_TAC THEN COND_CASES_TAC THEN SIMP_TAC hol_ss [])
+  SIMP_TAC arith_ss [BAG_IN, BAG_INN, BAG_INSERT] THEN
+  REPEAT GEN_TAC THEN COND_CASES_TAC THEN SIMP_TAC arith_ss [])
  before
  export_rewrites ["BAG_IN_BAG_INSERT"];
 
@@ -103,77 +109,65 @@ val BAG_INN_BAG_INSERT = store_thm(
   ``!b e1 e2:'a. BAG_INN e1 n (BAG_INSERT e2 b) =
                    BAG_INN e1 (n - 1) b /\ (e1 = e2) \/
                    BAG_INN e1 n b``,
-  SIMP_TAC hol_ss [BAG_INSERT, BAG_INN] THEN REPEAT GEN_TAC THEN
-  EQ_TAC THEN COND_CASES_TAC THEN STRIP_TAC THEN
-  ELIM_TAC THEN ASM_SIMP_TAC hol_ss []);
-
+  SRW_TAC [ARITH_ss][BAG_INSERT, BAG_INN]);
 
 val BAG_INN_BAG_INSERT_STRONG = store_thm (
   "BAG_INN_BAG_INSERT_STRONG",
    ``!b n e1 e2.
         BAG_INN e1 n (BAG_INSERT e2 b) =
           BAG_INN e1 (n - 1) b /\ (e1 = e2) \/
-          BAG_INN e1 n b /\ ~(e1 = e2)``,
+          BAG_INN e1 n b /\ e1 <> e2``,
   REWRITE_TAC [BAG_INN_BAG_INSERT] THEN
-  Cases_on `n` THEN SIMP_TAC hol_ss [BAG_INN_0] THEN
-  `n' < SUC n'` by bossLib.DECIDE_TAC THEN
+  SRW_TAC [][EQ_IMP_THM] THEN SRW_TAC [][] THEN
+  `(n = 0) \/ ?m. n = SUC m` by (Cases_on `n` THEN METIS_TAC []) THEN
+  SRW_TAC [][] THEN
+  `m < SUC m` by DECIDE_TAC THEN
   PROVE_TAC[BAG_INN_LESS]);
-
 
 val BAG_IN_BAG_UNION = Q.store_thm(
   "BAG_IN_BAG_UNION",
   `!b1 b2 e. BAG_IN e (BAG_UNION b1 b2) = BAG_IN e b1 \/ BAG_IN e b2`,
-  SIMP_TAC hol_ss [BAG_IN, BAG_UNION, BAG_INN]);
+  SRW_TAC [ARITH_ss][BAG_IN, BAG_UNION, BAG_INN]);
 val _ = export_rewrites ["BAG_IN_BAG_UNION"]
 
 val BAG_INN_BAG_UNION = Q.store_thm(
   "BAG_INN_BAG_UNION",
   `!n e b1 b2. BAG_INN e n (BAG_UNION b1 b2) =
                ?m1 m2. (n = m1 + m2) /\ BAG_INN e m1 b1 /\ BAG_INN e m2 b2`,
-  SIMP_TAC hol_ss [BAG_INN, BAG_UNION] THEN
-  REPEAT GEN_TAC THEN EQ_TAC THEN STRIP_TAC THEN ASM_SIMP_TAC hol_ss [] THEN
-  POP_ASSUM MP_TAC THEN Q.ID_SPEC_TAC `n` THEN
-  INDUCT_THEN numTheory.INDUCTION STRIP_ASSUME_TAC THENL [
-    SIMP_TAC hol_ss [],
-    REPEAT STRIP_TAC THEN
-    IMP_RES_TAC (ARITH_PROVE (Term`!n m. n >= SUC m ==> n >= m`)) THEN
-    FULL_SIMP_TAC hol_ss [] THEN
-    Q.SUBGOAL_THEN `b1 e > m1 \/ b2 e > m2` STRIP_ASSUME_TAC THENL [
-      myCONTR_TAC THEN FULL_SIMP_TAC hol_ss [],
-      MAP_EVERY Q.EXISTS_TAC [`SUC m1`, `m2`] THEN
-      ASM_SIMP_TAC hol_ss [],
-      MAP_EVERY Q.EXISTS_TAC [`m1`, `SUC m2`] THEN
-      ASM_SIMP_TAC hol_ss []
-    ]
+  SRW_TAC [ARITH_ss][BAG_INN, BAG_UNION, GREATER_EQ, EQ_IMP_THM] THEN
+  Induct_on `n` THEN1 SRW_TAC [][] THEN
+  STRIP_TAC THEN
+  `n <= b1 e + b2 e` by DECIDE_TAC THEN
+  FULL_SIMP_TAC (srw_ss()) [] THEN
+  `m1 < b1 e \/ m2 < b2 e` by DECIDE_TAC THENL [
+      MAP_EVERY Q.EXISTS_TAC [`SUC m1`, `m2`] THEN DECIDE_TAC,
+      MAP_EVERY Q.EXISTS_TAC [`m1`, `SUC m2`] THEN DECIDE_TAC
   ]);
 
 val BAG_INN_BAG_MERGE = Q.store_thm (
   "BAG_INN_BAG_MERGE",
   `!n e b1 b2. (BAG_INN e n (BAG_MERGE b1 b2)) =
                (BAG_INN e n b1 \/ BAG_INN e n b2)`,
-  SIMP_TAC hol_ss [BAG_INN, BAG_MERGE]);
+  SIMP_TAC arith_ss [BAG_INN, BAG_MERGE]);
 
 
 val BAG_IN_BAG_MERGE = Q.store_thm (
   "BAG_IN_BAG_MERGE",
   `!e b1 b2. (BAG_IN e (BAG_MERGE b1 b2)) =
              (BAG_IN e b1 \/ BAG_IN e b2)`,
-  SIMP_TAC hol_ss [BAG_IN, BAG_INN_BAG_MERGE]);
+  SIMP_TAC std_ss [BAG_IN, BAG_INN_BAG_MERGE]);
 
 val geq_refl = ARITH_PROVE ``m >= m``
 
 val BAG_EXTENSION = store_thm(
   "BAG_EXTENSION",
   ``!b1 b2. (b1 = b2) = (!n e:'a. BAG_INN e n b1 = BAG_INN e n b2)``,
-  CONV_TAC (DEPTH_CONV FUN_EQ_CONV) THEN REPEAT STRIP_TAC THEN
-  REWRITE_TAC [BAG_INN] THEN EQ_TAC THEN STRIP_TAC THENL [
-    REPEAT STRIP_TAC THEN ARWT,
-    GEN_TAC THEN REWRITE_TAC [
-      ARITH_PROVE ``(x = y) = (x >= y) /\ (y >= x)``
-    ] THEN CONJ_TAC THENL [
-      ASM_REWRITE_TAC [geq_refl],
-      POP_ASSUM (fn th => ASM_REWRITE_TAC [geq_refl, GSYM th])]
-    ]);
+  SRW_TAC [][BAG_INN, FUN_EQ_THM, GREATER_EQ] THEN
+  EQ_TAC THEN1 SRW_TAC [][] THEN
+  METIS_TAC [
+    ARITH_PROVE ``(x = y) = (x <= y) /\ (y <= x)``,
+    LESS_EQ_REFL
+  ]);
 
 val _ = print "Properties of BAG_INSERT\n"
 
@@ -182,81 +176,68 @@ val BAG_UNION_INSERT = Q.store_thm(
   `!e b1 b2.
      (BAG_UNION (BAG_INSERT e b1) b2 = BAG_INSERT e (BAG_UNION b1 b2)) /\
      (BAG_UNION b1 (BAG_INSERT e b2) = BAG_INSERT e (BAG_UNION b1 b2))`,
-  SIMP_TAC hol_ss [BAG_EXTENSION, BAG_INSERT, BAG_INN, BAG_UNION] THEN
-  REPEAT STRIP_TAC THEN COND_CASES_TAC THEN ASM_SIMP_TAC hol_ss []);
-
+  SRW_TAC [ARITH_ss][FUN_EQ_THM, BAG_INSERT, BAG_UNION] THEN
+  SRW_TAC [ARITH_ss][]);
 
 val BAG_INSERT_DIFF = store_thm (
   "BAG_INSERT_DIFF",
   ``!x b. ~(BAG_INSERT x b = b)``,
-  REPEAT GEN_TAC THEN
-  CONV_TAC (DEPTH_CONV FUN_EQ_CONV THENC NOT_FORALL_CONV) THEN
-  SIMP_TAC hol_ss [BAG_INSERT, aCOND_OUT_THM, fCOND_OUT_THM]);
+  SRW_TAC [COND_elim_ss][FUN_EQ_THM, BAG_INSERT]);
+val _ = export_rewrites ["BAG_INSERT_DIFF"]
 
 val BAG_INSERT_NOT_EMPTY = store_thm (
   "BAG_INSERT_NOT_EMPTY",
-  Term`!x b. ~(BAG_INSERT x b = EMPTY_BAG)`,
-  REPEAT GEN_TAC THEN
-  CONV_TAC (DEPTH_CONV FUN_EQ_CONV THENC NOT_FORALL_CONV) THEN
-  SIMP_TAC hol_ss [EMPTY_BAG_alt, BAG_INSERT, aCOND_OUT_THM,
-                   fCOND_OUT_THM] THEN MESON_TAC [])
-  before
-  export_rewrites ["BAG_INSERT_NOT_EMPTY"]
+  ``!x b. ~(BAG_INSERT x b = EMPTY_BAG)``,
+  SRW_TAC [COND_elim_ss][FUN_EQ_THM, BAG_INSERT, EMPTY_BAG, EXISTS_OR_THM]);
+val _ = export_rewrites ["BAG_INSERT_NOT_EMPTY"]
 
+val or_cong = REWRITE_RULE [GSYM AND_IMP_INTRO] OR_CONG
 val BAG_INSERT_ONE_ONE = store_thm(
   "BAG_INSERT_ONE_ONE",
   ``!b1 b2 x:'a.
       (BAG_INSERT x b1 = BAG_INSERT x b2) = (b1 = b2)``,
-  REPEAT STRIP_TAC THEN EQ_TAC THEN SIMP_TAC hol_ss [BAG_INSERT] THEN
-  CONV_TAC (DEPTH_CONV FUN_EQ_CONV) THEN REPEAT STRIP_TAC THEN
-  POP_ASSUM (MP_TAC o SPEC ``x':'a``) THEN
-  SIMP_TAC hol_ss [] THEN COND_CASES_TAC THEN
-  ASM_SIMP_TAC hol_ss []);
+  SIMP_TAC (srw_ss() ++ COND_elim_ss) [BAG_INSERT, FUN_EQ_THM, EQ_IMP_THM,
+                                       Cong or_cong, FORALL_AND_THM] THEN
+  METIS_TAC []);
+val _ = export_rewrites ["BAG_INSERT_ONE_ONE"]
 
 val C_BAG_INSERT_ONE_ONE = store_thm(
   "C_BAG_INSERT_ONE_ONE",
   ``!x y b. (BAG_INSERT x b = BAG_INSERT y b) = (x = y)``,
-  REPEAT STRIP_TAC THEN CONV_TAC (DEPTH_CONV FUN_EQ_CONV) THEN
-  EQ_TAC THENL [
-    DISCH_THEN (Q.SPEC_THEN `y` MP_TAC) THEN
-    SIMP_TAC hol_ss [BAG_INSERT] THEN COND_CASES_TAC THEN
-    ASM_SIMP_TAC hol_ss [],
-    DISCH_THEN SUBST1_TAC THEN GEN_TAC THEN REFL_TAC
-  ]);
+  SIMP_TAC (srw_ss() ++ COND_elim_ss ++ ARITH_ss)
+           [BAG_INSERT, FUN_EQ_THM, Cong or_cong] THEN
+  METIS_TAC []);
+val _ = export_rewrites ["C_BAG_INSERT_ONE_ONE"]
 
 val BAG_INSERT_commutes = store_thm(
   "BAG_INSERT_commutes",
   ``!b e1 e2. BAG_INSERT e1 (BAG_INSERT e2 b) =
                 BAG_INSERT e2 (BAG_INSERT e1 b)``,
-  REWRITE_TAC [BAG_EXTENSION] THEN
-  SIMP_TAC hol_ss [BAG_INN_BAG_INSERT] THEN
-  REPEAT STRIP_TAC THEN EQ_TAC THEN REPEAT STRIP_TAC THEN
-  ELIM_TAC THEN ARWT);
+  SIMP_TAC (srw_ss()) [BAG_INSERT, FUN_EQ_THM] THEN
+  REPEAT GEN_TAC THEN
+  REPEAT (COND_CASES_TAC THEN ASM_SIMP_TAC (srw_ss()) []) THEN
+  SRW_TAC [][]);
 
 val BAG_DECOMPOSE = store_thm
 ("BAG_DECOMPOSE",
  ``!e b. BAG_IN e b ==> ?b'. b = BAG_INSERT e b'``,
  REPEAT STRIP_TAC THEN
- Q.EXISTS_TAC `BAG_DIFF b {|e|}` THEN POP_ASSUM MP_TAC THEN
- RW_TAC hol_ss [BAG_INSERT,BAG_DIFF,EMPTY_BAG,FUN_EQ_THM,BAG_IN,BAG_INN] THEN
- RW_TAC hol_ss []);
+ Q.EXISTS_TAC `b - {|e|}` THEN POP_ASSUM MP_TAC THEN
+ SRW_TAC [ARITH_ss, COND_elim_ss]
+         [BAG_INSERT,BAG_DIFF,EMPTY_BAG,FUN_EQ_THM,BAG_IN,BAG_INN]);
 
 val _ = print "Properties of BAG_UNION\n";
 
 val BAG_UNION_LEFT_CANCEL = store_thm(
   "BAG_UNION_LEFT_CANCEL",
   ``!b b1 b2:'a -> num. (BAG_UNION b b1 = BAG_UNION b b2) = (b1 = b2)``,
-  REPEAT GEN_TAC THEN EQ_TAC THEN SIMP_TAC hol_ss [BAG_UNION] THEN
-  STRIP_TAC THEN CONV_TAC FUN_EQ_CONV THEN GEN_TAC THEN
-  POP_ASSUM (MP_TAC o C AP_THM ``x:'a``) THEN
-  SIMP_TAC hol_ss []);
+  SIMP_TAC arith_ss [BAG_UNION,FUN_EQ_THM]);
 val _ = export_rewrites ["BAG_UNION_LEFT_CANCEL"]
 
 val COMM_BAG_UNION = store_thm(
   "COMM_BAG_UNION",
   ``!b1 b2. BAG_UNION b1 b2 = BAG_UNION b2 b1``,
-  REWRITE_TAC [BAG_UNION] THEN
-  REPEAT STRIP_TAC THEN FUN_EQ_TAC THEN SIMP_TAC hol_ss []);
+  SRW_TAC [ARITH_ss][BAG_UNION, FUN_EQ_THM]);
 val bu_comm = COMM_BAG_UNION;
 
 val BAG_UNION_RIGHT_CANCEL = store_thm(
@@ -265,15 +246,21 @@ val BAG_UNION_RIGHT_CANCEL = store_thm(
   METIS_TAC [bu_comm, BAG_UNION_LEFT_CANCEL]);
 val _ = export_rewrites ["BAG_UNION_RIGHT_CANCEL"]
 
-
-
 val ASSOC_BAG_UNION = store_thm(
   "ASSOC_BAG_UNION",
   ``!b1 b2 b3. BAG_UNION b1 (BAG_UNION b2 b3)
                  =
                  BAG_UNION (BAG_UNION b1 b2) b3``,
-  REWRITE_TAC [BAG_UNION] THEN
-  REPEAT STRIP_TAC THEN FUN_EQ_TAC THEN SIMP_TAC hol_ss []);
+  SRW_TAC [ARITH_ss][BAG_UNION, FUN_EQ_THM]);
+
+val BAG_UNION_EMPTY = store_thm(
+  "BAG_UNION_EMPTY",
+  ``(!b. b + {||} = b) /\
+    (!b. {||} + b = b) /\
+    (!b1 b2. (b1 + b2 = {||}) = (b1 = {||}) /\ (b2 = {||}))``,
+  SRW_TAC [][BAG_UNION, EMPTY_BAG, FUN_EQ_THM] THEN METIS_TAC []);
+val _ =  export_rewrites ["BAG_UNION_EMPTY"]
+
 
 val _ = print "Definition and properties of BAG_DELETE\n"
 val BAG_DELETE = new_definition (
@@ -283,7 +270,7 @@ val BAG_DELETE = new_definition (
 val BAG_DELETE_EMPTY = store_thm(
   "BAG_DELETE_EMPTY",
   ``!(e:'a) b. ~(BAG_DELETE EMPTY_BAG e b)``,
-  SIMP_TAC hol_ss [BAG_DELETE] THEN
+  SIMP_TAC std_ss [BAG_DELETE] THEN
   ACCEPT_TAC (GSYM BAG_INSERT_NOT_EMPTY));
 
 val BAG_DELETE_commutes = store_thm(
@@ -291,7 +278,7 @@ val BAG_DELETE_commutes = store_thm(
   ``!b0 b1 b2 e1 e2:'a.
          BAG_DELETE b0 e1 b1 /\ BAG_DELETE b1 e2 b2 ==>
          ?b'. BAG_DELETE b0 e2 b' /\ BAG_DELETE b' e1 b2``,
-  SIMP_TAC hol_ss [BAG_DELETE] THEN
+  SIMP_TAC std_ss [BAG_DELETE] THEN
   ACCEPT_TAC BAG_INSERT_commutes);
 
 val BAG_DELETE_11 = store_thm(
@@ -299,40 +286,40 @@ val BAG_DELETE_11 = store_thm(
   ``!b0 (e1:'a) e2 b1 b2.
          BAG_DELETE b0 e1 b1 /\ BAG_DELETE b0 e2 b2 ==>
          ((e1 = e2) = (b1 = b2))``,
-  REWRITE_TAC [BAG_DELETE] THEN REPEAT STRIP_TAC THEN EQ_TAC THEN
-  STRIP_TAC THEN ELIM_TAC THENL [
-    IMP_RES_TAC BAG_INSERT_ONE_ONE THEN ARWT,
-    IMP_RES_TAC C_BAG_INSERT_ONE_ONE THEN ARWT
-  ]);
+  SRW_TAC [][BAG_DELETE, EQ_IMP_THM] THEN
+  FULL_SIMP_TAC (srw_ss()) []);
 
 val BAG_INN_BAG_DELETE = store_thm(
   "BAG_INN_BAG_DELETE",
   Term`!b n e. BAG_INN e n b /\ n > 0 ==> ?b'. BAG_DELETE b e b'`,
-  SIMP_TAC hol_ss [BAG_INN, BAG_DELETE, BAG_INSERT] THEN
-  REPEAT STRIP_TAC THEN CONV_TAC (DEPTH_CONV FUN_EQ_CONV) THEN
-  SIMP_TAC hol_ss [fCOND_OUT_THM, aCOND_OUT_THM] THEN
-  EXISTS_TAC ``\x. if x = e then b e - 1 else b x`` THEN
-  ASM_SIMP_TAC hol_ss []);
+  SRW_TAC [][BAG_DELETE] THEN MATCH_MP_TAC BAG_DECOMPOSE THEN
+  SRW_TAC [][BAG_IN] THEN
+  `(n = 1) \/ 1 < n` by DECIDE_TAC THEN
+  METIS_TAC [BAG_INN_LESS]);
 
 val BAG_IN_BAG_DELETE = store_thm(
   "BAG_IN_BAG_DELETE",
   Term`!b e:'a. BAG_IN e b ==> ?b'. BAG_DELETE b e b'`,
-  MESON_TAC [BAG_INN_BAG_DELETE, ARITH_PROVE (Term`1 > 0`), BAG_IN]);
+  METIS_TAC [BAG_INN_BAG_DELETE, ARITH_PROVE (Term`1 > 0`), BAG_IN]);
+
+val ELIM_TAC = BasicProvers.VAR_EQ_TAC
+val ARWT = SRW_TAC [ARITH_ss][]
+open mesonLib
 
 val BAG_DELETE_INSERT = Q.store_thm(
   "BAG_DELETE_INSERT",
   `!x y b1 b2.
       BAG_DELETE (BAG_INSERT x b1) y b2 ==>
       (x = y) /\ (b1 = b2) \/ (?b3. BAG_DELETE b1 y b3) /\ ~(x = y)`,
-  SIMP_TAC hol_ss [BAG_DELETE] THEN REPEAT STRIP_TAC THEN
+  SIMP_TAC std_ss [BAG_DELETE] THEN REPEAT STRIP_TAC THEN
   Q.ASM_CASES_TAC `x = y` THEN ARWT THENL [
-    FULL_SIMP_TAC hol_ss [BAG_INSERT_ONE_ONE],
+    FULL_SIMP_TAC std_ss [BAG_INSERT_ONE_ONE],
     Q.SUBGOAL_THEN `BAG_IN y b1`
       (STRIP_ASSUME_TAC o
        MATCH_MP (REWRITE_RULE [BAG_DELETE] BAG_IN_BAG_DELETE))
     THENL [
       ASM_MESON_TAC [BAG_IN_BAG_INSERT],
-      ELIM_TAC THEN SIMP_TAC hol_ss [BAG_INSERT_ONE_ONE]
+      ELIM_TAC THEN SIMP_TAC std_ss [BAG_INSERT_ONE_ONE]
     ]
   ]);
 
@@ -348,34 +335,83 @@ val BAG_DELETE_BAG_IN_down = store_thm(
   ``!b0 b e1 e2:'a.
          BAG_DELETE b0 e1 b /\ ~(e1 = e2) /\ BAG_IN e2 b0 ==>
          BAG_IN e2 b``,
-  SIMP_TAC hol_ss [BAG_DELETE, BAG_IN_BAG_INSERT, LEFT_AND_OVER_OR,
+  SIMP_TAC std_ss [BAG_DELETE, BAG_IN_BAG_INSERT, LEFT_AND_OVER_OR,
                    DISJ_IMP_THM]);
 
 val BAG_DELETE_BAG_IN = store_thm(
   "BAG_DELETE_BAG_IN",
   ``!b0 b e:'a. BAG_DELETE b0 e b ==> BAG_IN e b0``,
-  SIMP_TAC hol_ss [BAG_IN_BAG_INSERT, BAG_DELETE]);
+  SIMP_TAC std_ss [BAG_IN_BAG_INSERT, BAG_DELETE]);
 
 val BAG_DELETE_concrete = store_thm(
   "BAG_DELETE_concrete",
   ``!b0 b e. BAG_DELETE b0 e b =
                b0 e > 0 /\ (b = \x. if (x = e) then b0 e - 1 else b0 x)``,
-  REPEAT STRIP_TAC THEN REWRITE_TAC [BAG_DELETE, BAG_INSERT] THEN EQ_TAC
-  THEN STRIP_TAC THEN ELIM_TAC THEN
-  CONV_TAC (DEPTH_CONV FUN_EQ_CONV) THEN
-  ASM_SIMP_TAC hol_ss [fCOND_OUT_THM, aCOND_OUT_THM]);
+  SRW_TAC [ARITH_ss][FUN_EQ_THM, BAG_DELETE, BAG_INSERT, EQ_IMP_THM] THEN
+  SRW_TAC [][]);
+
+val add_eq_conv_diff = prove(
+  ``(M + {|a|} = N + {|b|}) =
+    (M = N) /\ (a = b) \/
+    (M = N - {|a|} + {|b|}) /\ (N = M - {|b|} + {|a|})``,
+  SRW_TAC [][BAG_UNION, BAG_DIFF, FUN_EQ_THM, BAG_INSERT, EMPTY_BAG] THEN
+  Cases_on `a = b` THEN SRW_TAC [][] THENL [
+    EQ_TAC THEN1 SRW_TAC [][] THEN STRIP_TAC THEN
+    Q.X_GEN_TAC `x` THEN
+    REPEAT (POP_ASSUM (Q.SPEC_THEN `x` MP_TAC)) THEN SRW_TAC [][] THEN
+    DECIDE_TAC,
+
+    EQ_TAC THEN STRIP_TAC THEN REPEAT CONJ_TAC THEN
+    Q.X_GEN_TAC `x` THEN
+    REPEAT (FIRST_X_ASSUM (Q.SPEC_THEN `x` MP_TAC)) THEN
+    SRW_TAC [][] THEN DECIDE_TAC
+  ]);
+
+val insert_diffM2 = prove(
+  ``BAG_IN x M ==> (M - {|x|} + {|x|} = M)``,
+  SRW_TAC [][BAG_UNION, BAG_DIFF, BAG_INSERT, EMPTY_BAG, FUN_EQ_THM, BAG_IN,
+             BAG_INN] THEN
+  SRW_TAC [][] THEN DECIDE_TAC);
+
+val BAG_UNION_DIFF_eliminate = store_thm(
+  "BAG_UNION_DIFF_eliminate",
+  ``(BAG_DIFF (BAG_UNION b c) c = b) /\
+    (BAG_DIFF (BAG_UNION c b) c = b)``,
+  SRW_TAC [][BAG_DIFF, BAG_UNION, FUN_EQ_THM]);
+val _ = export_rewrites ["BAG_UNION_DIFF_eliminate"]
+
+val add_eq_conv_ex = prove(
+  ``(M + {|a|} = N + {|b|}) =
+    (M = N) /\ (a = b) \/
+    ?k. (M = k + {|b|}) /\ (N = k + {|a|})``,
+  SRW_TAC [][add_eq_conv_diff] THEN Cases_on `a = b` THENL [
+    SRW_TAC [][EQ_IMP_THM] THEN
+    FULL_SIMP_TAC (srw_ss()) [insert_diffM2] THEN
+    POP_ASSUM ACCEPT_TAC,
+
+    SRW_TAC [][] THEN EQ_TAC THEN STRIP_TAC THENL [
+      POP_ASSUM SUBST_ALL_TAC THEN SRW_TAC [][] THEN
+      `BAG_IN b M` by METIS_TAC [BAG_IN_BAG_UNION, BAG_IN_BAG_INSERT] THEN
+      SRW_TAC [][insert_diffM2],
+
+      SRW_TAC [][]
+    ]
+  ]);
+
+val BAG_INSERT_EQUAL = save_thm(
+  "BAG_INSERT_EQUAL",
+  SIMP_RULE (srw_ss()) [BAG_UNION_INSERT] add_eq_conv_ex)
 
 val BAG_DELETE_TWICE = store_thm(
   "BAG_DELETE_TWICE",
   ``!b0 e1 e2 b1 b2.
          BAG_DELETE b0 e1 b1 /\ BAG_DELETE b0 e2 b2 /\ ~(b1 = b2) ==>
          ?b. BAG_DELETE b1 e2 b /\ BAG_DELETE b2 e1 b``,
-  REPEAT STRIP_TAC THEN
-  Q.SUBGOAL_THEN `~(e1 = e2)` ASSUME_TAC THENL [
-    ASM_MESON_TAC [BAG_DELETE_11],
-    FULL_SIMP_TAC hol_ss [BAG_DELETE_concrete]
-  ] THEN FUN_EQ_TAC THEN ASM_SIMP_TAC hol_ss [] THEN
-  REPEAT COND_CASES_TAC THEN RWT THEN ELIM_TAC THEN RWT);
+  SRW_TAC [][BAG_DELETE] THEN
+  `b2 + {|e2|} = b1 + {|e1|}` by SRW_TAC [][BAG_UNION_INSERT] THEN
+  POP_ASSUM (STRIP_ASSUME_TAC o REWRITE_RULE [add_eq_conv_ex]) THEN
+  FULL_SIMP_TAC (srw_ss()) [] THEN
+  SRW_TAC [][BAG_UNION_INSERT]);
 
 val SING_BAG = new_definition(
   "SING_BAG",
@@ -390,33 +426,15 @@ val EL_BAG = new_definition(
   "EL_BAG",
   ``EL_BAG (e:'a) = BAG_INSERT e EMPTY_BAG``);
 
-val EL_BAG_11 = Q.store_thm(
+val EL_BAG_11 = store_thm(
   "EL_BAG_11",
-  `!x y. (EL_BAG x = EL_BAG y) ==> (x = y)`,
-  SIMP_TAC hol_ss [EL_BAG, BAG_INSERT, EMPTY_BAG] THEN
-  REPEAT GEN_TAC THEN CONV_TAC (DEPTH_CONV FUN_EQ_CONV) THEN
-  SIMP_TAC hol_ss [] THEN
-  DISCH_THEN (Q.SPEC_THEN `y` MP_TAC) THEN SIMP_TAC hol_ss [] THEN
-  SIMP_TAC hol_ss [aCOND_OUT_THM, fCOND_OUT_THM]);
+  ``!x y. (EL_BAG x = EL_BAG y) ==> (x = y)``,
+  SRW_TAC [][EL_BAG]);
 
-val EL_BAG_INSERT_squeeze0 = prove(
-  Term`!x b y. (EL_BAG x = BAG_INSERT y b) ==> (b = EMPTY_BAG)`,
-  SIMP_TAC hol_ss [EL_BAG, BAG_INSERT, EMPTY_BAG] THEN
-  REPEAT GEN_TAC THEN
-  DISCH_THEN (ASSUME_TAC o SIMP_RULE hol_ss [FUN_EQ_THM]) THEN
-  FUN_EQ_TAC THEN SIMP_TAC hol_ss [] THEN
-  FIRST_ASSUM (Q.SPEC_THEN `x'` MP_TAC) THEN
-  REPEAT COND_CASES_TAC THEN ELIM_TAC THEN SIMP_TAC hol_ss [] THEN
-  FIRST_ASSUM
-    (Q.SPEC_THEN `y`
-                 (MP_TAC o SIMP_RULE hol_ss [Q.ASSUME `~(x = y)`])) THEN
-  SIMP_TAC hol_ss []);
-
-val EL_BAG_INSERT_squeeze = Q.store_thm(
+val EL_BAG_INSERT_squeeze = store_thm(
   "EL_BAG_INSERT_squeeze",
-  `!x b y. (EL_BAG x = BAG_INSERT y b) ==> (x = y) /\ (b = EMPTY_BAG)`,
-  REPEAT STRIP_TAC THEN IMP_RES_TAC EL_BAG_INSERT_squeeze0 THEN
-  ASM_MESON_TAC [EL_BAG, EL_BAG_11]);
+  ``!x b y. (EL_BAG x = BAG_INSERT y b) ==> (x = y) /\ (b = EMPTY_BAG)``,
+  SIMP_TAC (srw_ss()) [EL_BAG, BAG_INSERT_EQUAL]);
 
 val SING_EL_BAG = store_thm(
   "SING_EL_BAG",
@@ -426,24 +444,14 @@ val SING_EL_BAG = store_thm(
 val BAG_INSERT_UNION = store_thm(
   "BAG_INSERT_UNION",
   ``!b e. BAG_INSERT e b = BAG_UNION (EL_BAG e) b``,
-  REPEAT GEN_TAC THEN FUN_EQ_TAC THEN
-  SIMP_TAC hol_ss [
-    BAG_UNION, BAG_INSERT, EL_BAG, EMPTY_BAG] THEN
-  COND_CASES_TAC THEN ELIM_TAC THEN SIMP_TAC hol_ss []);
+  SRW_TAC [][EL_BAG, BAG_UNION_INSERT]);
 
-val one_equal =
-  ARITH_PROVE (Term`(1 = n + m) = (n = 1) /\ (m = 0) \/ (m = 1) /\ (n = 0)`)
 val BAG_INSERT_EQ_UNION = Q.store_thm(
   "BAG_INSERT_EQ_UNION",
   `!e b1 b2 b. (BAG_INSERT e b = BAG_UNION b1 b2) ==>
                BAG_IN e b1 \/ BAG_IN e b2`,
-  SIMP_TAC hol_ss [BAG_EXTENSION, BAG_INN_BAG_UNION, BAG_IN,
-                   BAG_INN_BAG_INSERT] THEN
-  REPEAT STRIP_TAC THEN
-  POP_ASSUM (Q.SPECL_THEN [`1`, `e`]
-                          (STRIP_ASSUME_TAC o
-                           SIMP_RULE hol_ss [BAG_INN_0, one_equal])) THEN
-  ELIM_TAC THEN ASM_SIMP_TAC hol_ss []);
+  REPEAT STRIP_TAC THEN POP_ASSUM (MP_TAC o Q.AP_TERM `BAG_IN e`) THEN
+  SRW_TAC [][]);
 
 val BAG_DELETE_SING = store_thm(
   "BAG_DELETE_SING",
@@ -453,45 +461,40 @@ val BAG_DELETE_SING = store_thm(
 val NOT_IN_EMPTY_BAG = store_thm(
   "NOT_IN_EMPTY_BAG",
   ``!x:'a. ~(BAG_IN x EMPTY_BAG)``,
-  SIMP_TAC hol_ss [BAG_IN, BAG_INN, EMPTY_BAG])
-  before
-  export_rewrites ["NOT_IN_EMPTY_BAG"];
+  SIMP_TAC std_ss [BAG_IN, BAG_INN, EMPTY_BAG])
+val _ = export_rewrites ["NOT_IN_EMPTY_BAG"];
 
 val BAG_INN_EMPTY_BAG = Q.store_thm(
   "BAG_INN_EMPTY_BAG",
   `!e n. BAG_INN e n EMPTY_BAG = (n = 0)`,
-  SIMP_TAC hol_ss [BAG_INN, EMPTY_BAG, EQ_IMP_THM])
-  before
-  export_rewrites ["BAG_INN_EMPTY_BAG"];
+  SIMP_TAC arith_ss [BAG_INN, EMPTY_BAG, EQ_IMP_THM])
+val _ = export_rewrites ["BAG_INN_EMPTY_BAG"];
 
 val MEMBER_NOT_EMPTY = store_thm(
   "MEMBER_NOT_EMPTY",
   ``!b. (?x. BAG_IN x b) = ~(b = EMPTY_BAG)``,
-  SIMP_TAC hol_ss [BAG_IN,BAG_INN,EMPTY_BAG_alt] THEN
-  CONV_TAC (DEPTH_CONV FUN_EQ_CONV) THEN
-  SIMP_TAC hol_ss [ARITH_PROVE ``(x >= 1) = ~(x = 0)``]);
+  METIS_TAC [BAG_cases, BAG_IN_BAG_INSERT, NOT_IN_EMPTY_BAG]);
 
 val _ = print "Properties of SUB_BAG\n"
-val geq_lemma = prove(
-  ``(!n. a >= n ==> b >= n) = (b >= a)``,
-  EQ_TAC THENL [
-    DISCH_THEN (SPEC ``a:num`` >- SIMP_RULE hol_ss [] >-
-                ASSUME_TAC) THEN carwt,
-    REPEAT STRIP_TAC THEN ASM_SIMP_TAC hol_ss []
+
+val _ = overload_on ("<=", ``SUB_BAG``)
+val _ = overload_on ("<", ``PSUB_BAG``)
+val _ = send_to_back_overload "<=" {Name = "SUB_BAG", Thy = "bag"}
+val _ = send_to_back_overload "<" {Name = "PSUB_BAG", Thy = "bag"}
+
+val SUB_BAG_LEQ = store_thm (
+  "SUB_BAG_LEQ",
+  ``SUB_BAG b1 b2 = !x. b1 x <= b2 x``,
+  SRW_TAC [][SUB_BAG, BAG_INN, EQ_IMP_THM] THENL [
+    POP_ASSUM (Q.SPECL_THEN [`x`, `b1 x`] MP_TAC) THEN DECIDE_TAC,
+    FIRST_X_ASSUM (Q.SPEC_THEN `x` MP_TAC) THEN DECIDE_TAC
   ]);
-val ZGTN = ARITH_PROVE (Term`!n. 0 >= n = (n = 0)`)
 
 val SUB_BAG_EMPTY = store_thm (
   "SUB_BAG_EMPTY",
-  ``(!b:'a->num. SUB_BAG EMPTY_BAG b) /\
-      (!b:'a->num. SUB_BAG b EMPTY_BAG = (b = EMPTY_BAG))``,
-  REPEAT STRIP_TAC THEN
-  SIMP_TAC hol_ss [EMPTY_BAG, SUB_BAG, BAG_INN, geq_lemma] THEN
-  EQ_TAC THEN STRIP_TAC THENL [
-    FUN_EQ_TAC THEN
-    POP_ASSUM (fn th => SIMP_TAC hol_ss [SPEC_ALL th]),
-    ELIM_TAC THEN SIMP_TAC hol_ss []
-  ]);
+  ``(!b:'a->num. SUB_BAG {||} b) /\
+    (!b:'a->num. SUB_BAG b {||} = (b = {||}))``,
+  SRW_TAC [][SUB_BAG_LEQ, EMPTY_BAG, FUN_EQ_THM]);
 
 val SUB_BAG_REFL = store_thm(
   "SUB_BAG_REFL",
@@ -506,11 +509,8 @@ val PSUB_BAG_IRREFL = store_thm(
 val SUB_BAG_ANTISYM = store_thm(
   "SUB_BAG_ANTISYM",
   ``!(b1:'a -> num) b2. SUB_BAG b1 b2 /\ SUB_BAG b2 b1 ==> (b1 = b2)``,
-  REWRITE_TAC [SUB_BAG, BAG_INN] THEN REPEAT STRIP_TAC THEN
-  FUN_EQ_TAC THEN
-  MATCH_MP_TAC arithmeticTheory.LESS_EQUAL_ANTISYM THEN
-  REWRITE_TAC [ARITH_PROVE ``x <= y = y >= x``] THEN
-  CONJ_TAC THEN FIRST_ASSUM MATCH_MP_TAC THEN CONV_TAC ARITH_CONV);
+  SRW_TAC [][SUB_BAG_LEQ, FUN_EQ_THM,
+             DECIDE ``(x:num = y) <=> x <= y /\ y <= x``]);
 
 val PSUB_BAG_ANTISYM = store_thm(
   "PSUB_BAG_ANTISYM",
@@ -520,100 +520,62 @@ val PSUB_BAG_ANTISYM = store_thm(
 val SUB_BAG_TRANS = store_thm(
   "SUB_BAG_TRANS",
   ``!b1 b2 b3. SUB_BAG (b1:'a->num) b2 /\ SUB_BAG b2 b3 ==>
-                 SUB_BAG b1 b3``,
+               SUB_BAG b1 b3``,
   MESON_TAC [SUB_BAG, BAG_INN]);
 
 val PSUB_BAG_TRANS = store_thm(
   "PSUB_BAG_TRANS",
   ``!(b1:'a -> num) b2 b3. PSUB_BAG b1 b2 /\ PSUB_BAG b2 b3 ==>
-                             PSUB_BAG b1 b3``,
+                           PSUB_BAG b1 b3``,
   MESON_TAC [PSUB_BAG, SUB_BAG_TRANS, SUB_BAG_ANTISYM]);
-
 
 val PSUB_BAG_SUB_BAG = store_thm(
   "PSUB_BAG_SUB_BAG",
   ``!(b1:'a->num) b2. PSUB_BAG b1 b2 ==> SUB_BAG b1 b2``,
-  SIMP_TAC hol_ss [PSUB_BAG]);
+  SIMP_TAC std_ss [PSUB_BAG]);
 
 val PSUB_BAG_NOT_EQ = store_thm(
   "PSUB_BAG_NOT_EQ",
   ``!(b1:'a -> num) b2. PSUB_BAG b1 b2 ==> ~(b1 = b2)``,
-  SIMP_TAC hol_ss [PSUB_BAG]);
-
-val SUB_BAG_LEQ = store_thm(
-  "SUB_BAG_LEQ",
-  ``!b1 b2:'a -> num. SUB_BAG b1 b2 = !x. b1 x <= b2 x``,
-  SIMP_TAC hol_ss [SUB_BAG, BAG_INN, geq_lemma] THEN
-  SIMP_TAC hol_ss [arithmeticTheory.GREATER_EQ]);
+  SIMP_TAC std_ss [PSUB_BAG]);
 
 val _ = print "Properties of BAG_DIFF\n";
 
 val BAG_DIFF_EMPTY = store_thm(
   "BAG_DIFF_EMPTY",
-  ``(!b. BAG_DIFF b b = EMPTY_BAG) /\
-     (!b. BAG_DIFF b EMPTY_BAG = b) /\
-     (!b. BAG_DIFF EMPTY_BAG b = EMPTY_BAG) /\
-     (!b1 b2.
-        SUB_BAG b1 b2 ==> (BAG_DIFF b1 b2 = EMPTY_BAG))``,
-  SIMP_TAC hol_ss [BAG_DIFF,EMPTY_BAG,SUB_BAG,BAG_INN,geq_lemma] THEN
-  REPEAT STRIP_TAC THEN FUN_EQ_TAC THEN
-  ASSUM_LIST (fn thl => SIMP_TAC hol_ss (map SPEC_ALL thl)));
+  ``(!b. b - b = {||}) /\
+    (!b. b - {||} = b) /\
+    (!b. {||} - b = {||}) /\
+    (!b1 b2.
+        b1 <= b2 ==> (b1 - b2 = {||}))``,
+  SRW_TAC [][SUB_BAG_LEQ, BAG_DIFF, EMPTY_BAG, FUN_EQ_THM]);
 
 val BAG_DIFF_EMPTY_simple = save_thm(
   "BAG_DIFF_EMPTY_simple",
   LIST_CONJ (List.take(CONJUNCTS BAG_DIFF_EMPTY, 3)))
-  before
-  export_rewrites ["BAG_DIFF_EMPTY_simple"];
+val _ = export_rewrites ["BAG_DIFF_EMPTY_simple"];
 
-val BAG_DIFF_INSERT_same = Q.store_thm(
+val BAG_DIFF_INSERT_same = store_thm(
   "BAG_DIFF_INSERT_same",
-  `!x b1 b2. BAG_DIFF (BAG_INSERT x b1) (BAG_INSERT x b2) =
-             BAG_DIFF b1 b2`,
-  SIMP_TAC hol_ss [BAG_DIFF, SUB_BAG, BAG_INN, geq_lemma,
-                   BAG_INSERT] THEN
-  REPEAT GEN_TAC THEN FUN_EQ_TAC THEN SIMP_TAC hol_ss [] THEN
-  COND_CASES_TAC THEN ASM_SIMP_TAC hol_ss [])
-  before
-  export_rewrites ["BAG_DIFF_INSERT_same"];
+  ``!x b1 b2. BAG_DIFF (BAG_INSERT x b1) (BAG_INSERT x b2) =
+             BAG_DIFF b1 b2``,
+  SRW_TAC [COND_elim_ss, ARITH_ss][BAG_DIFF, FUN_EQ_THM, BAG_INSERT]);
+val _ = export_rewrites ["BAG_DIFF_INSERT_same"];
 
 val BAG_DIFF_INSERT = Q.store_thm(
   "BAG_DIFF_INSERT",
   `!x b1 b2.
-      ~(BAG_IN x b1) ==>
+      ~BAG_IN x b1 ==>
       (BAG_DIFF (BAG_INSERT x b2) b1 = BAG_INSERT x (BAG_DIFF b2 b1))`,
-  SIMP_TAC hol_ss [BAG_DIFF, SUB_BAG, BAG_INN, geq_lemma,
-                   BAG_INSERT, BAG_IN] THEN REPEAT STRIP_TAC THEN
-  FUN_EQ_TAC THEN SIMP_TAC hol_ss [] THEN COND_CASES_TAC THEN
-  ASM_SIMP_TAC hol_ss []);
+  SRW_TAC [COND_elim_ss, ARITH_ss][FUN_EQ_THM, BAG_DIFF, BAG_INSERT,
+                                   Cong or_cong, BAG_IN, BAG_INN]);
 
 val NOT_IN_BAG_DIFF = Q.store_thm(
   "NOT_IN_BAG_DIFF",
-  `!x b1 b2. ~(BAG_IN x b1) ==>
+  `!x b1 b2. ~BAG_IN x b1 ==>
             (BAG_DIFF b1 (BAG_INSERT x b2) = BAG_DIFF b1 b2)`,
-  SIMP_TAC hol_ss [BAG_INSERT, BAG_DIFF, BAG_IN, BAG_INN, BAG_EXTENSION,
-                   ZGTN, aCOND_OUT_THM, fCOND_OUT_THM]);
-
-val BAG_UNION_DIFF_eliminate = store_thm(
-  "BAG_UNION_DIFF_eliminate",
-  ``(BAG_DIFF (BAG_UNION b c) c = b) /\
-    (BAG_DIFF (BAG_UNION c b) c = b)``,
-  SRW_TAC [][BAG_DIFF, BAG_UNION, FUN_EQ_THM]);
-val _ = export_rewrites ["BAG_UNION_DIFF_eliminate"]
-
-val BAG_UNION_EMPTY = store_thm(
-  "BAG_UNION_EMPTY",
-  ``(!b. BAG_UNION b EMPTY_BAG = b) /\
-     (!b. BAG_UNION EMPTY_BAG b = b) /\
-     (!b1 b2. (BAG_UNION b1 b2 = EMPTY_BAG) =
-              (b1 = EMPTY_BAG) /\ (b2 = EMPTY_BAG))``,
-  SIMP_TAC (hol_ss ++ ETA_ss) [BAG_UNION, EMPTY_BAG] THEN
-  REPEAT STRIP_TAC THEN EQ_TAC THEN
-  DISCH_THEN (REPEAT_TCL STRIP_THM_THEN (CONV_RULE FUN_EQ_CONV >-
-              SIMP_RULE hol_ss [] >- ASSUME_TAC)) THEN
-  REPEAT STRIP_TAC THEN FUN_EQ_TAC THEN
-  ASSUM_LIST (fn thl => SIMP_TAC hol_ss (map SPEC_ALL thl)))
-  before
-  export_rewrites ["BAG_UNION_EMPTY"]
+  SRW_TAC [COND_elim_ss, ARITH_ss][FUN_EQ_THM, BAG_IN, BAG_INN, BAG_INSERT,
+                                   BAG_DIFF]);
 
 val BAG_UNION_DIFF = store_thm(
   "BAG_UNION_DIFF",
@@ -621,38 +583,36 @@ val BAG_UNION_DIFF = store_thm(
         SUB_BAG Z Y ==>
         (BAG_UNION X (BAG_DIFF Y Z) = BAG_DIFF (BAG_UNION X Y) Z) /\
         (BAG_UNION (BAG_DIFF Y Z) X = BAG_DIFF (BAG_UNION X Y) Z)``,
-  SIMP_TAC hol_ss [BAG_UNION,BAG_INN,SUB_BAG,BAG_DIFF,geq_lemma] THEN
-  REPEAT STRIP_TAC THEN FUN_EQ_TAC THEN
-  POP_ASSUM (fn th => SIMP_TAC hol_ss [SPEC_ALL th]));
+  SRW_TAC [][SUB_BAG_LEQ, BAG_UNION, BAG_DIFF, FUN_EQ_THM] THEN
+  POP_ASSUM (fn th => SIMP_TAC arith_ss [SPEC_ALL th]));
 
 val BAG_DIFF_2L = store_thm(
   "BAG_DIFF_2L",
   ``!X Y Z:'a->num.
          BAG_DIFF (BAG_DIFF X Y) Z = BAG_DIFF X (BAG_UNION Y Z)``,
-  SIMP_TAC hol_ss [BAG_UNION,BAG_INN,SUB_BAG,BAG_DIFF]);
+  SIMP_TAC arith_ss [BAG_UNION,BAG_INN,SUB_BAG,BAG_DIFF]);
 
 val BAG_DIFF_2R = store_thm(
   "BAG_DIFF_2R",
   ``!A B C:'a->num.
          SUB_BAG C B  ==>
          (BAG_DIFF A (BAG_DIFF B C) = BAG_DIFF (BAG_UNION A C) B)``,
-  SIMP_TAC hol_ss [BAG_UNION,BAG_INN,SUB_BAG,BAG_DIFF,geq_lemma] THEN
-  REPEAT STRIP_TAC THEN FUN_EQ_TAC THEN
-  ASSUM_LIST (fn thl => SIMP_TAC hol_ss (map SPEC_ALL thl)));
+  SRW_TAC [][BAG_UNION, BAG_DIFF, SUB_BAG_LEQ, FUN_EQ_THM] THEN
+  ASSUM_LIST (fn thl => SIMP_TAC arith_ss (map SPEC_ALL thl)));
 
+val std_ss = arith_ss
 val SUB_BAG_BAG_DIFF = store_thm(
   "SUB_BAG_BAG_DIFF",
   ``!X Y Y' Z W:'a->num.
         SUB_BAG (BAG_DIFF X Y) (BAG_DIFF Z W) ==>
         SUB_BAG (BAG_DIFF X (BAG_UNION Y Y'))
                 (BAG_DIFF Z (BAG_UNION W Y'))``,
-  SIMP_TAC hol_ss [
-    BAG_DIFF, SUB_BAG, BAG_INN, BAG_UNION, geq_lemma, ZGTN,
+  SIMP_TAC std_ss [
+    BAG_DIFF, SUB_BAG_LEQ, BAG_INN, BAG_UNION,
     DISJ_IMP_THM] THEN
   REPEAT STRIP_TAC THEN
-  FIRST_ASSUM (Q.SPECL [`x:'a`, `n + Y' x`] >-
-               SIMP_RULE hol_ss [] >- STRIP_ASSUME_TAC) THEN
-  ASM_SIMP_TAC hol_ss []);
+  FIRST_ASSUM (Q.SPEC_THEN `x` (STRIP_ASSUME_TAC o SIMP_RULE std_ss [])) THEN
+  ASM_SIMP_TAC std_ss []);
 
 local
   fun bdf (b1, b2) (b3, b4) =
@@ -670,8 +630,9 @@ in
           ^(bdf ("b1", "b2") ("b3", "b1")) /\
           ^(bdf ("b2", "b1") ("b1", "b3")) /\
           ^(bdf ("b2", "b1") ("b3", "b1"))``,
-    REPEAT STRIP_TAC THEN FUN_EQ_TAC THEN
-    SIMP_TAC hol_ss [BAG_DIFF, BAG_UNION])
+    REPEAT STRIP_TAC THEN
+    SIMP_TAC std_ss [BAG_DIFF, BAG_UNION, FUN_EQ_THM])
+  val _ = export_rewrites ["BAG_DIFF_UNION_eliminate"]
 end;
 
 local
@@ -690,36 +651,22 @@ in
           ^(bdf ("b1", "b2") ("b3", "b1")) /\
           ^(bdf ("b2", "b1") ("b1", "b3")) /\
           ^(bdf ("b2", "b1") ("b3", "b1"))``,
-    SIMP_TAC hol_ss [SUB_BAG, BAG_UNION, BAG_INN] THEN
-    REWRITE_TAC [geq_lemma] THEN REPEAT STRIP_TAC THEN EQ_TAC THEN
+    SIMP_TAC std_ss [SUB_BAG_LEQ, BAG_UNION, BAG_INN] THEN
+    REPEAT STRIP_TAC THEN EQ_TAC THEN
     STRIP_TAC THEN
-    POP_ASSUM (fn th => SIMP_TAC hol_ss [SPEC_ALL th]))
+    POP_ASSUM (fn th => SIMP_TAC std_ss [SPEC_ALL th]))
+  val _ = export_rewrites ["SUB_BAG_UNION_eliminate"]
 end;
 
 val move_BAG_UNION_over_eq = store_thm(
   "move_BAG_UNION_over_eq",
   ``!X Y Z:'a->num. (BAG_UNION X Y = Z) ==> (X = BAG_DIFF Z Y)``,
-  SIMP_TAC (hol_ss ++ ETA_ss) [BAG_UNION, BAG_DIFF]);
-
-val COMM_BAG_UNION = store_thm(
-  "COMM_BAG_UNION",
-  ``!b1 b2. BAG_UNION b1 b2 = BAG_UNION b2 b1``,
-  REWRITE_TAC [BAG_UNION] THEN
-  REPEAT STRIP_TAC THEN FUN_EQ_TAC THEN SIMP_TAC hol_ss []);
-val bu_comm = COMM_BAG_UNION;
-
-val ASSOC_BAG_UNION = store_thm(
-  "ASSOC_BAG_UNION",
-  ``!b1 b2 b3. BAG_UNION b1 (BAG_UNION b2 b3)
-                 =
-                 BAG_UNION (BAG_UNION b1 b2) b3``,
-  REWRITE_TAC [BAG_UNION] THEN
-  REPEAT STRIP_TAC THEN FUN_EQ_TAC THEN SIMP_TAC hol_ss []);
+  SIMP_TAC (std_ss ++ ETA_ss) [BAG_UNION, BAG_DIFF]);
 
 val std_bag_tac =
-  SIMP_TAC hol_ss [BAG_UNION, SUB_BAG, BAG_INN, geq_lemma] THEN
+  SIMP_TAC std_ss [BAG_UNION, SUB_BAG_LEQ, BAG_INN] THEN
   REPEAT STRIP_TAC THEN
-  ASSUM_LIST (fn thl => SIMP_TAC hol_ss (map SPEC_ALL thl))
+  ASSUM_LIST (fn thl => SIMP_TAC std_ss (map SPEC_ALL thl))
 
 fun bag_thm t = prove(Term t, std_bag_tac);
 
@@ -795,49 +742,27 @@ val SUB_BAG_UNION = save_thm(
 val SUB_BAG_EL_BAG = Q.store_thm(
   "SUB_BAG_EL_BAG",
   `!e b. SUB_BAG (EL_BAG e) b = BAG_IN e b`,
-  SIMP_TAC (hol_ss ++ impnorm_set) [EL_BAG, BAG_IN, SUB_BAG,
-    BAG_INN_BAG_INSERT, FORALL_AND_THM, BAG_INN_EMPTY_BAG,
-    BAG_INN_0, ARITH_PROVE (Term`!n. (n - 1 = 0) = (n = 0) \/ (n = 1)`)]);
-
-val GREATER_OR_EQ_TRANS =
-  ARITH_PROVE (Term`!n m q. n >= m /\ m >= q ==> n >= q`)
+  SRW_TAC [COND_elim_ss, ARITH_ss]
+          [SUB_BAG_LEQ, EL_BAG, BAG_IN, BAG_INN, BAG_INSERT, EMPTY_BAG]);
 
 val SUB_BAG_INSERT = Q.store_thm(
   "SUB_BAG_INSERT",
   `!e b1 b2. SUB_BAG (BAG_INSERT e b1) (BAG_INSERT e b2) =
-              SUB_BAG b1 b2`,
-  SIMP_TAC (hol_ss ++ impnorm_set) [SUB_BAG, BAG_INN_BAG_INSERT,
-    FORALL_AND_THM, BAG_INN, geq_lemma,
-    ARITH_PROVE
-      (Term`!x n. (x >= n - 1) \/ (x >= n) = (x >= n - 1)`)] THEN
-  REPEAT GEN_TAC THEN EQ_TAC THEN REPEAT STRIP_TAC THENL [
-    Q.ASM_CASES_TAC `x = e` THENL [
-      ELIM_TAC THEN
-      FIRST_X_ASSUM (tofl (concl >- dest_forall >-
-                           fst >- type_of >- curry op= (Type`:num`)) >-
-        Q.SPEC `m + 1` >-
-        SIMP_RULE hol_ss [] >- GEN_ALL >-
-        SIMP_RULE hol_ss [geq_lemma] >- ACCEPT_TAC),
-      FIRST_X_ASSUM (tofl (concl >- dest_forall >- fst >- type_of >-
-        curry op= (Type`:'a`)) >- Q.SPEC `x` >-
-        SIMP_RULE hol_ss [Q.ASSUME `~(x = e)`, geq_lemma] >-
-        ACCEPT_TAC)
-    ],
-    ASM_MESON_TAC [GREATER_OR_EQ_TRANS],
-    ASM_MESON_TAC [GREATER_OR_EQ_TRANS]
-  ]);
+             SUB_BAG b1 b2`,
+  SRW_TAC [ARITH_ss][BAG_INSERT, SUB_BAG_LEQ, EQ_IMP_THM] THEN
+  POP_ASSUM (Q.SPEC_THEN `x` MP_TAC) THEN SRW_TAC [ARITH_ss][]);
 
 val NOT_IN_SUB_BAG_INSERT = Q.store_thm(
   "NOT_IN_SUB_BAG_INSERT",
   `!b1 b2 e. ~(BAG_IN e b1) ==>
              (SUB_BAG b1 (BAG_INSERT e b2) = SUB_BAG b1 b2)`,
-  SIMP_TAC hol_ss [SUB_BAG, BAG_INN_BAG_INSERT, BAG_IN] THEN
+  SIMP_TAC std_ss [SUB_BAG, BAG_INN_BAG_INSERT, BAG_IN] THEN
   REPEAT STRIP_TAC THEN EQ_TAC THEN REPEAT STRIP_TAC THENL [
     RES_TAC THEN ELIM_TAC THEN
     STRIP_ASSUME_TAC (ARITH_PROVE (Term`(n = 0) \/ (n = 1) \/ (1 < n)`))
     THENL [
-      FULL_SIMP_TAC hol_ss [],
-      FULL_SIMP_TAC hol_ss [],
+      FULL_SIMP_TAC std_ss [],
+      FULL_SIMP_TAC std_ss [],
       ASM_MESON_TAC [BAG_INN_LESS]
     ],
     ASM_MESON_TAC []
@@ -846,19 +771,18 @@ val NOT_IN_SUB_BAG_INSERT = Q.store_thm(
 val SUB_BAG_BAG_IN = Q.store_thm(
   "SUB_BAG_BAG_IN",
   `!x b1 b2. SUB_BAG (BAG_INSERT x b1) b2 ==> BAG_IN x b2`,
-  SIMP_TAC hol_ss [SUB_BAG, BAG_INSERT, BAG_IN, BAG_INN, geq_lemma] THEN
+  SIMP_TAC std_ss [SUB_BAG_LEQ, BAG_INSERT, BAG_IN, BAG_INN] THEN
   REPEAT GEN_TAC THEN
-  DISCH_THEN (Q.SPEC `x` >- SIMP_RULE hol_ss [] >- ASSUME_TAC) THEN
-  ASM_SIMP_TAC hol_ss []);
+  DISCH_THEN (Q.SPEC_THEN `x` (ASSUME_TAC o SIMP_RULE std_ss [])) THEN
+  ASM_SIMP_TAC std_ss []);
 
 val SUB_BAG_EXISTS = store_thm(
   "SUB_BAG_EXISTS",
   ``!b1 b2:'a->num. SUB_BAG b1 b2 = ?b. b2 = BAG_UNION b1 b``,
-  REPEAT STRIP_TAC THEN EQ_TAC THEN STRIP_TAC THENL [
-    FULL_SIMP_TAC hol_ss [SUB_BAG, BAG_INN, geq_lemma, BAG_UNION] THEN
-    Q.EXISTS_TAC `\x. b2 x - b1 x` THEN FUN_EQ_TAC THEN
-    POP_ASSUM (fn th => SIMP_TAC hol_ss [SPEC_ALL th]),
-    ELIM_TAC THEN SIMP_TAC hol_ss [SUB_BAG_UNION, SUB_BAG_REFL]
+  SRW_TAC [][SUB_BAG_LEQ, BAG_UNION, FUN_EQ_THM, EQ_IMP_THM] THENL [
+    Q.EXISTS_TAC `\x. b2 x - b1 x` THEN
+    POP_ASSUM (fn th => SIMP_TAC std_ss [SPEC_ALL th]),
+    ASM_SIMP_TAC std_ss []
   ]);
 
 val SUB_BAG_UNION_DIFF = store_thm(
@@ -867,21 +791,17 @@ val SUB_BAG_UNION_DIFF = store_thm(
          SUB_BAG b1 b3 ==>
          (SUB_BAG b2 (BAG_DIFF b3 b1) = SUB_BAG (BAG_UNION b1 b2) b3)
   ``,
-  SIMP_TAC hol_ss [SUB_BAG,BAG_INN,geq_lemma,BAG_DIFF,BAG_UNION] THEN
-  REPEAT STRIP_TAC THEN EQ_TAC THEN REPEAT STRIP_TAC THENL [
-    POP_ASSUM (Q.SPECL [`x`, `b2 x`] >- SIMP_RULE hol_ss [] >-
-               STRIP_ASSUME_TAC) THEN
-    FULL_SIMP_TAC hol_ss [ARITH_PROVE (Term`!n. 0 >= n = (n = 0)`)],
-    ASSUM_LIST (SIMP_TAC hol_ss o map SPEC_ALL)
-  ]);
+  SIMP_TAC std_ss [SUB_BAG_LEQ,BAG_DIFF,BAG_UNION] THEN
+  REPEAT STRIP_TAC THEN EQ_TAC THEN REPEAT STRIP_TAC THEN
+  REPEAT (POP_ASSUM (MP_TAC o SPEC_ALL)) THEN DECIDE_TAC);
 
 val SUB_BAG_UNION_down = store_thm(
   "SUB_BAG_UNION_down",
   ``!b1 b2 b3:'a->num. SUB_BAG (BAG_UNION b1 b2) b3 ==>
                         SUB_BAG b1 b3 /\ SUB_BAG b2 b3``,
-  SIMP_TAC hol_ss [BAG_UNION, SUB_BAG, BAG_INN, geq_lemma] THEN
+  SIMP_TAC std_ss [BAG_UNION, SUB_BAG_LEQ] THEN
   REPEAT STRIP_TAC THEN
-  ASSUM_LIST (fn thl => SIMP_TAC hol_ss (map SPEC_ALL thl)));
+  ASSUM_LIST (fn thl => SIMP_TAC std_ss (map SPEC_ALL thl)));
 
 val SUB_BAG_DIFF = store_thm(
   "SUB_BAG_DIFF",
@@ -891,80 +811,14 @@ val SUB_BAG_DIFF = store_thm(
          SUB_BAG b2 b1 ==> SUB_BAG b4 b3 ==>
          (SUB_BAG (BAG_DIFF b1 b2) (BAG_DIFF b3 b4) =
           SUB_BAG (BAG_UNION b1 b4) (BAG_UNION b2 b3)))``,
-  SIMP_TAC hol_ss [BAG_DIFF, BAG_UNION, SUB_BAG, BAG_INN,
-                   geq_lemma, ZGTN] THEN REPEAT STRIP_TAC THEN
-  TRY EQ_TAC  THEN REPEAT STRIP_TAC THEN
-  ASSUM_LIST (fn thl => SIMP_TAC hol_ss (map SPEC_ALL thl)) THEN
-  POP_ASSUM_LIST (List.rev >- MAP_EVERY (Q.SPEC `x` >- ASSUME_TAC)) THEN
-  POP_ASSUM (Q.SPEC `b1 x - b2 x` >- MP_TAC) THEN
-  ASM_SIMP_TAC hol_ss []);
-
-val BAG_delta = new_definition (
-  "BAG_delta",
-  ``BAG_delta (B1:'a->num, B2) B3 =
-     BAG_DIFF (BAG_UNION B3 (BAG_DIFF B2 B1)) (BAG_DIFF B1 B2)``);
-
-val SUB_BAG_delta = store_thm(
-  "SUB_BAG_delta",
-  ``(!A B0 B:'a -> num.
-        SUB_BAG B0 A ==> SUB_BAG B (BAG_delta (B0, B) A)) /\
-     (!A B0 B:'a -> num.
-        SUB_BAG A B0 ==> SUB_BAG (BAG_delta (B0, B) A) B)``,
-  REWRITE_TAC [BAG_delta, SUB_BAG, geq_lemma, BAG_INN, BAG_DIFF,
-               BAG_UNION] THEN REPEAT STRIP_TAC THEN BETA_TAC THEN
-  ASM_CASES_TAC ``B (x:'a) >= B0 x`` THEN
-  ASM_SIMP_TAC boolSimps.bool_ss
-                (map ARITH_PROVE [``x >= y ==> (y - x = 0)``,
-                                  ``~(x >= y) ==> (x - y = 0)``,
-                                  ``x - 0 = x``,
-                                  ``x + 0 = x``]) THEN
-  ASSUM_LIST (fn thl => SIMP_TAC hol_ss (map SPEC_ALL thl)));
-
-val BAG_delta_rm_lemma = prove(
-  ``!A BU BD X:'a->num.
-         SUB_BAG X A ==>
-         (BAG_delta (A, BAG_DIFF (BAG_UNION A BU) BD) X =
-          BAG_DIFF (BAG_UNION X BU) BD)``,
-  REWRITE_TAC [BAG_delta] THEN
-  SIMP_TAC hol_ss [BAG_DIFF_2L, BAG_DIFF_2R, SUB_BAG_DIFF,
-                    SUB_BAG_UNION, BAG_UNION_DIFF,
-                    BAG_DIFF_UNION_eliminate] THEN
-  REWRITE_TAC [SUB_BAG, BAG_INN, geq_lemma, BAG_DIFF, BAG_UNION,
-               BAG_delta] THEN REPEAT STRIP_TAC THEN FUN_EQ_TAC THEN
-  SIMP_TAC boolSimps.bool_ss [] THEN
-  ASM_CASES_TAC ``BU (x:'a) >= BD x`` THENL [
-    ASM_SIMP_TAC boolSimps.bool_ss
-                  (map ARITH_PROVE [``x >= y ==>
-                                       ((a + x) - y = a + (x - y))``,
-                                    ``x - (x + y) = 0``,
-                                    ``x - 0 = x``]),
-    ASM_SIMP_TAC boolSimps.bool_ss
-                  (map ARITH_PROVE [``~(x >= y) ==> (x - y = 0)``,
-                                    ``x + 0 = x``]) THEN
-    ASM_CASES_TAC ``A (x:'a) + BU x >= BD x`` THENL [
-      ASM_SIMP_TAC
-        boolSimps.bool_ss
-        (map ARITH_PROVE [``x >= y ==> (z - (x - y) = (z + y) - x)``,
-                          ``(x + y) - (x + z) = y - z``]) THEN
-      ASM_SIMP_TAC hol_ss [],
-      ASM_SIMP_TAC boolSimps.bool_ss
-                    (map ARITH_PROVE [``~(x >= y) ==> (x - y = 0)``,
-                                      ``x + 0 = x``]) THEN
-      ASSUM_LIST (fn thl => SIMP_TAC hol_ss (map SPEC_ALL thl))
-    ]
-  ]);
-
-val BAG_delta_eliminate = save_thm(
-  "BAG_delta_eliminate",
-  CONJ BAG_delta_rm_lemma
-       (ONCE_REWRITE_RULE [bu_comm] BAG_delta_rm_lemma));
+  SRW_TAC [ARITH_ss][BAG_DIFF, BAG_UNION, SUB_BAG_LEQ, EQ_IMP_THM] THEN
+  REPEAT (POP_ASSUM (MP_TAC o SPEC_ALL)) THEN DECIDE_TAC);
 
 val SUB_BAG_PSUB_BAG = store_thm(
   "SUB_BAG_PSUB_BAG",
   ``!(b1:'a -> num) b2.
          SUB_BAG b1 b2 = PSUB_BAG b1 b2 \/ (b1 = b2)``,
-  REPEAT GEN_TAC THEN EQ_TAC THEN
-  SIMP_TAC hol_ss [PSUB_BAG, DISJ_IMP_THM, SUB_BAG_REFL])
+  METIS_TAC [PSUB_BAG, SUB_BAG_REFL]);
 
 val mono_cond = COND_RAND
 val mono_cond2 = COND_RATOR
@@ -972,7 +826,7 @@ val mono_cond2 = COND_RATOR
 val BAG_DELETE_PSUB_BAG = store_thm(
   "BAG_DELETE_PSUB_BAG",
   ``!b0 (e:'a) b. BAG_DELETE b0 e b ==> PSUB_BAG b b0``,
-  SIMP_TAC hol_ss [BAG_DELETE, SUB_BAG, PSUB_BAG, BAG_INSERT_DIFF,
+  SIMP_TAC std_ss [BAG_DELETE, SUB_BAG, PSUB_BAG, BAG_INSERT_DIFF,
                     BAG_INN_BAG_INSERT]);
 
 val _ = print "Relating bags to (pred)sets\n";
@@ -989,82 +843,74 @@ val BAG_OF_SET = new_definition(
 val SET_OF_EMPTY = store_thm (
   "SET_OF_EMPTY",
   ``BAG_OF_SET (EMPTY:'a->bool) = EMPTY_BAG``,
-  FUN_EQ_TAC THEN
-  SIMP_TAC hol_ss [BAG_OF_SET, EMPTY_BAG, NOT_IN_EMPTY])
-  before
-  export_rewrites ["SET_OF_EMPTY"];
+  SIMP_TAC (srw_ss()) [BAG_OF_SET, EMPTY_BAG, FUN_EQ_THM])
+val _ = export_rewrites ["SET_OF_EMPTY"];
 
 val BAG_OF_EMPTY = store_thm (
   "BAG_OF_EMPTY",
   ``SET_OF_BAG (EMPTY_BAG:'a->num) = EMPTY``,
-  FUN_EQ_TAC THEN
-  SIMP_TAC hol_ss [SET_OF_BAG, NOT_IN_EMPTY_BAG, EMPTY_DEF])
- before
- export_rewrites ["BAG_OF_EMPTY"]
+  SIMP_TAC std_ss [FUN_EQ_THM, SET_OF_BAG, NOT_IN_EMPTY_BAG, EMPTY_DEF])
+val _ = export_rewrites ["BAG_OF_EMPTY"]
 
 val SET_BAG_I = store_thm (
   "SET_BAG_I",
   ``!s:'a->bool. SET_OF_BAG (BAG_OF_SET s) = s``,
-  GEN_TAC THEN FUN_EQ_TAC THEN
-  SIMP_TAC hol_ss [BAG_OF_SET, SET_OF_BAG, mono_cond, mono_cond2,
-                    BAG_IN, BAG_INN, SPECIFICATION]);
+  SRW_TAC [][SET_OF_BAG, BAG_OF_SET, FUN_EQ_THM, BAG_IN, BAG_INN, IN_DEF] THEN
+  SRW_TAC [][]);
+val _ = export_rewrites ["SET_BAG_I"]
 
 val SUB_BAG_SET = store_thm (
   "SUB_BAG_SET",
   ``!b1 b2:'a->num.
         SUB_BAG b1 b2 ==> (SET_OF_BAG b1) SUBSET (SET_OF_BAG b2)``,
-  SIMP_TAC hol_ss [SUB_BAG, SET_OF_BAG, BAG_IN, SPECIFICATION,
+  SIMP_TAC std_ss [SUB_BAG, SET_OF_BAG, BAG_IN, SPECIFICATION,
                     SUBSET_DEF]);
 
 val SET_OF_BAG_UNION = store_thm(
   "SET_OF_BAG_UNION",
   ``!b1 b2:'a->num. SET_OF_BAG (BAG_UNION b1 b2) =
                       SET_OF_BAG b1 UNION SET_OF_BAG b2``,
-  REWRITE_TAC [SET_OF_BAG, BAG_IN, UNION_DEF, BAG_UNION, BAG_INN,
-               SPECIFICATION] THEN REPEAT GEN_TAC THEN FUN_EQ_TAC THEN
-  SIMP_TAC hol_ss [] THEN
-  CONV_TAC (rhs_CONV (ONCE_REWRITE_CONV [GSYM SPECIFICATION])) THEN
-  SIMP_TAC hol_ss [GSPECIFICATION]);
+  SRW_TAC [][SET_OF_BAG, EXTENSION] THEN SRW_TAC [][IN_DEF]);
 
 val SET_OF_BAG_MERGE = store_thm (
   "SET_OF_BAG_MERGE",
   ``!b1 b2. SET_OF_BAG (BAG_MERGE b1 b2) =
             SET_OF_BAG b1 UNION SET_OF_BAG b2``,
   ONCE_REWRITE_TAC[EXTENSION] THEN
-  SIMP_TAC hol_ss [SET_OF_BAG, IN_UNION, IN_ABS,
+  SIMP_TAC std_ss [SET_OF_BAG, IN_UNION, IN_ABS,
 		   BAG_IN_BAG_MERGE]);
 
 val SET_OF_BAG_INSERT = Q.store_thm(
   "SET_OF_BAG_INSERT",
   `!e b. SET_OF_BAG (BAG_INSERT e b) = e INSERT (SET_OF_BAG b)`,
-  SIMP_TAC hol_ss [SET_OF_BAG, BAG_INSERT, INSERT_DEF, BAG_IN,
+  SIMP_TAC std_ss [SET_OF_BAG, BAG_INSERT, INSERT_DEF, BAG_IN,
                     EXTENSION, GSPECIFICATION, BAG_INN] THEN
-  SIMP_TAC hol_ss [SPECIFICATION] THEN REPEAT GEN_TAC THEN
-  COND_CASES_TAC THEN SIMP_TAC hol_ss []);
+  SIMP_TAC std_ss [SPECIFICATION] THEN REPEAT GEN_TAC THEN
+  COND_CASES_TAC THEN SIMP_TAC std_ss []);
 
 val SET_OF_EL_BAG = Q.store_thm(
   "SET_OF_EL_BAG",
   `!e. SET_OF_BAG (EL_BAG e) = {e}`,
-  SIMP_TAC hol_ss [EL_BAG, SET_OF_BAG_INSERT, BAG_OF_EMPTY]);
+  SIMP_TAC std_ss [EL_BAG, SET_OF_BAG_INSERT, BAG_OF_EMPTY]);
 
 val SET_OF_BAG_DIFF_SUBSET_down = Q.store_thm(
   "SET_OF_BAG_DIFF_SUBSET_down",
   `!b1 b2. (SET_OF_BAG b1) DIFF (SET_OF_BAG b2) SUBSET
             SET_OF_BAG (BAG_DIFF b1 b2)`,
-  SIMP_TAC hol_ss [SUBSET_DEF, IN_DIFF, BAG_DIFF, SET_OF_BAG, BAG_IN,
+  SIMP_TAC std_ss [SUBSET_DEF, IN_DIFF, BAG_DIFF, SET_OF_BAG, BAG_IN,
                     BAG_INN] THEN
-  SIMP_TAC hol_ss [SPECIFICATION]);
+  SIMP_TAC std_ss [SPECIFICATION]);
 
 val SET_OF_BAG_DIFF_SUBSET_up = Q.store_thm(
   "SET_OF_BAG_DIFF_SUBSET_up",
   `!b1 b2. SET_OF_BAG (BAG_DIFF b1 b2) SUBSET SET_OF_BAG b1`,
-  SIMP_TAC hol_ss [SUBSET_DEF, BAG_DIFF, SET_OF_BAG, BAG_IN, BAG_INN]
-  THEN SIMP_TAC hol_ss [SPECIFICATION]);
+  SIMP_TAC std_ss [SUBSET_DEF, BAG_DIFF, SET_OF_BAG, BAG_IN, BAG_INN]
+  THEN SIMP_TAC std_ss [SPECIFICATION]);
 
 val IN_SET_OF_BAG = Q.store_thm(
   "IN_SET_OF_BAG",
   `!x b. x IN SET_OF_BAG b = BAG_IN x b`,
-  SIMP_TAC hol_ss [SET_OF_BAG, SPECIFICATION])
+  SIMP_TAC std_ss [SET_OF_BAG, SPECIFICATION])
  before
  export_rewrites ["IN_SET_OF_BAG"];
 
@@ -1094,16 +940,16 @@ val BAG_DISJOINT_DIFF = store_thm(
   "BAG_DISJOINT_DIFF",
   ``!B1 B2:'a->num.
       BAG_DISJOINT (BAG_DIFF B1 B2) (BAG_DIFF B2 B1)``,
-  SIMP_TAC hol_ss [INTER_DEF, DISJOINT_DEF, BAG_DISJOINT, BAG_DIFF,
+  SIMP_TAC std_ss [INTER_DEF, DISJOINT_DEF, BAG_DISJOINT, BAG_DIFF,
                     SET_OF_BAG, BAG_IN, BAG_INN, EXTENSION,
                     GSPECIFICATION, NOT_IN_EMPTY] THEN
-  SIMP_TAC hol_ss [SPECIFICATION]);
+  SIMP_TAC std_ss [SPECIFICATION]);
 
 val BAG_DISJOINT_BAG_IN = store_thm (
   "BAG_DISJOINT_BAG_IN",
   ``!b1 b2. BAG_DISJOINT b1 b2 =
             !e. ~(BAG_IN e b1) \/ ~(BAG_IN e b2)``,
-  SIMP_TAC hol_ss [BAG_DISJOINT, DISJOINT_DEF,
+  SIMP_TAC std_ss [BAG_DISJOINT, DISJOINT_DEF,
  		   EXTENSION, NOT_IN_EMPTY,
 		   IN_INTER, IN_SET_OF_BAG]);
 
@@ -1115,7 +961,7 @@ val BAG_DISJOINT_BAG_INSERT = store_thm (
     (!b1 b2 e2.
       BAG_DISJOINT b1 (BAG_INSERT e2 b2) =
       (~(BAG_IN e2 b1) /\ (BAG_DISJOINT b1 b2)))``,
-  SIMP_TAC hol_ss [BAG_DISJOINT_BAG_IN,
+  SIMP_TAC std_ss [BAG_DISJOINT_BAG_IN,
 		   BAG_IN_BAG_INSERT] THEN
   METIS_TAC[]);
 
@@ -1130,7 +976,7 @@ val FINITE_BAG = Q.new_definition(
 val FINITE_EMPTY_BAG = Q.store_thm(
   "FINITE_EMPTY_BAG",
   `FINITE_BAG EMPTY_BAG`,
-  SIMP_TAC hol_ss [FINITE_BAG]);
+  SIMP_TAC std_ss [FINITE_BAG]);
 
 val FINITE_BAG_INSERT = Q.store_thm(
   "FINITE_BAG_INSERT",
@@ -1142,44 +988,36 @@ val FINITE_BAG_INDUCT = Q.store_thm(
   `!P. P EMPTY_BAG /\
         (!b. P b ==> (!e. P (BAG_INSERT e b))) ==>
         (!b. FINITE_BAG b ==> P b)`,
-  SIMP_TAC hol_ss [FINITE_BAG]);
+  SIMP_TAC std_ss [FINITE_BAG]);
 
 val STRONG_FINITE_BAG_INDUCT = save_thm(
   "STRONG_FINITE_BAG_INDUCT",
-  (Q.SPEC `\b. FINITE_BAG b /\ P b` >-
-   SIMP_RULE hol_ss [FINITE_EMPTY_BAG, FINITE_BAG_INSERT] >-
-   GEN_ALL) FINITE_BAG_INDUCT)
+  FINITE_BAG_INDUCT
+      |> Q.SPEC `\b. FINITE_BAG b /\ P b`
+      |> SIMP_RULE std_ss [FINITE_EMPTY_BAG, FINITE_BAG_INSERT]
+      |> GEN_ALL)
 
 val FINITE_BAG_INSERT_down' = prove(
-  Term`!b. FINITE_BAG b ==> (!e b0. (b = BAG_INSERT e b0) ==> FINITE_BAG b0)`,
+  ``!b. FINITE_BAG b ==> (!e b0. (b = BAG_INSERT e b0) ==> FINITE_BAG b0)``,
   HO_MATCH_MP_TAC STRONG_FINITE_BAG_INDUCT THEN
-  SIMP_TAC hol_ss [BAG_INSERT_NOT_EMPTY] THEN
+  SIMP_TAC std_ss [BAG_INSERT_NOT_EMPTY] THEN
   REPEAT STRIP_TAC THEN Q.ASM_CASES_TAC `e = e'` THENL [
     ELIM_TAC THEN IMP_RES_TAC BAG_INSERT_ONE_ONE THEN ELIM_TAC THEN
-    ASM_SIMP_TAC hol_ss [],
+    ASM_SIMP_TAC std_ss [],
     ALL_TAC
   ] THEN Q.SUBGOAL_THEN `?b'. b = BAG_INSERT e' b'` STRIP_ASSUME_TAC
   THENL [
-    SIMP_TAC hol_ss [GSYM BAG_DELETE] THEN
+    SIMP_TAC std_ss [GSYM BAG_DELETE] THEN
     MATCH_MP_TAC BAG_IN_BAG_DELETE THEN
-    Q.SUBGOAL_THEN `BAG_IN e' (BAG_INSERT e b)`
-      (REWRITE_RULE [BAG_IN_BAG_INSERT] >- STRIP_ASSUME_TAC)
-    THENL [
-      ARWT THEN ASM_REWRITE_TAC [BAG_IN_BAG_INSERT],
-      FULL_SIMP_TAC hol_ss []
-    ],
+    FULL_SIMP_TAC (srw_ss()) [BAG_INSERT_EQUAL],
     RES_TAC THEN ELIM_TAC THEN
     RULE_ASSUM_TAC (ONCE_REWRITE_RULE [BAG_INSERT_commutes]) THEN
-    IMP_RES_TAC BAG_INSERT_ONE_ONE THEN ELIM_TAC THEN
-    ASM_MESON_TAC [FINITE_BAG_INSERT]
+    FULL_SIMP_TAC (srw_ss()) [] THEN SRW_TAC [][FINITE_BAG_INSERT]
   ])
-
-val FINITE_BAG_INSERT_down =
-  SIMP_RULE hol_ss [RIGHT_IMP_FORALL_THM] FINITE_BAG_INSERT_down'
 
 val FINITE_BAG_INSERT = prove(
   Term`!e b. FINITE_BAG (BAG_INSERT e b) = FINITE_BAG b`,
-  MESON_TAC [FINITE_BAG_INSERT, FINITE_BAG_INSERT_down])
+  MESON_TAC [FINITE_BAG_INSERT, FINITE_BAG_INSERT_down'])
 
 val FINITE_BAG_THM = save_thm(
   "FINITE_BAG_THM",
@@ -1187,16 +1025,15 @@ val FINITE_BAG_THM = save_thm(
  before
  export_rewrites ["FINITE_BAG_THM"];
 
-
 val FINITE_BAG_DIFF = Q.store_thm(
   "FINITE_BAG_DIFF",
   `!b1. FINITE_BAG b1 ==> !b2. FINITE_BAG (BAG_DIFF b1 b2)`,
   HO_MATCH_MP_TAC STRONG_FINITE_BAG_INDUCT THEN
-  SIMP_TAC hol_ss [BAG_DIFF_EMPTY, FINITE_BAG_THM] THEN
+  SIMP_TAC std_ss [BAG_DIFF_EMPTY, FINITE_BAG_THM] THEN
   REPEAT STRIP_TAC THEN Q.ASM_CASES_TAC `BAG_IN e b2` THENL [
     IMP_RES_TAC (REWRITE_RULE [BAG_DELETE] BAG_IN_BAG_DELETE) THEN
-    ASM_SIMP_TAC hol_ss [BAG_DIFF_INSERT_same],
-    ASM_SIMP_TAC hol_ss [BAG_DIFF_INSERT, FINITE_BAG_THM]
+    ASM_SIMP_TAC std_ss [BAG_DIFF_INSERT_same],
+    ASM_SIMP_TAC std_ss [BAG_DIFF_INSERT, FINITE_BAG_THM]
   ]);
 
 val FINITE_BAG_DIFF_dual = Q.store_thm(
@@ -1215,23 +1052,16 @@ val FINITE_BAG_UNION_1 = prove(
   Term`!b1. FINITE_BAG b1 ==>
             !b2. FINITE_BAG b2 ==> FINITE_BAG (BAG_UNION b1 b2)`,
   HO_MATCH_MP_TAC STRONG_FINITE_BAG_INDUCT THEN
-  SIMP_TAC hol_ss [FINITE_BAG_THM, BAG_UNION_EMPTY, BAG_UNION_INSERT]);
+  SIMP_TAC std_ss [FINITE_BAG_THM, BAG_UNION_EMPTY, BAG_UNION_INSERT]);
 val FINITE_BAG_UNION_2 = prove(
-  Term`!b. FINITE_BAG b ==>
-           !b1 b2. (b = BAG_UNION b1 b2) ==> FINITE_BAG b1 /\ FINITE_BAG b2`,
-  HO_MATCH_MP_TAC STRONG_FINITE_BAG_INDUCT THEN
-  CONJ_TAC THENL [
-    REPEAT GEN_TAC THEN CONV_TAC (ant_CONV (REWR_CONV EQ_SYM_EQ)) THEN
-    SIMP_TAC hol_ss [BAG_UNION_EMPTY, FINITE_BAG_THM],
-    REPEAT (GEN_TAC ORELSE myDISCH_TAC) THEN
-    MAP_EVERY IMP_RES_TAC [BAG_INSERT_EQ_UNION,
-                           REWRITE_RULE [BAG_DELETE] BAG_IN_BAG_DELETE] THEN
-    ELIM_TAC THEN
-    FULL_SIMP_TAC hol_ss [BAG_UNION_INSERT, BAG_INSERT_ONE_ONE,
-                          FINITE_BAG_THM] THEN
-    FIRST_ASSUM MATCH_MP_TAC THEN REWRITE_TAC []
-  ]);
-
+  ``!b. FINITE_BAG b ==>
+           !b1 b2. (b = BAG_UNION b1 b2) ==> FINITE_BAG b1 /\ FINITE_BAG b2``,
+  HO_MATCH_MP_TAC STRONG_FINITE_BAG_INDUCT THEN SRW_TAC [][] THEN
+  MAP_EVERY IMP_RES_TAC [BAG_INSERT_EQ_UNION,
+                         REWRITE_RULE [BAG_DELETE] BAG_IN_BAG_DELETE] THEN
+  ELIM_TAC THEN
+  FULL_SIMP_TAC std_ss [BAG_UNION_INSERT, BAG_INSERT_ONE_ONE,
+                        FINITE_BAG_THM] THEN METIS_TAC []);
 
 val FINITE_BAG_UNION = Q.store_thm(
   "FINITE_BAG_UNION",
@@ -1244,13 +1074,12 @@ val FINITE_SUB_BAG = Q.store_thm(
   "FINITE_SUB_BAG",
   `!b1. FINITE_BAG b1 ==> !b2. SUB_BAG b2 b1 ==> FINITE_BAG b2`,
   HO_MATCH_MP_TAC STRONG_FINITE_BAG_INDUCT THEN
-  SIMP_TAC hol_ss [SUB_BAG_EMPTY, FINITE_BAG_THM] THEN
+  SIMP_TAC std_ss [SUB_BAG_EMPTY, FINITE_BAG_THM] THEN
   REPEAT STRIP_TAC THEN Q.ASM_CASES_TAC `BAG_IN e b2` THENL [
     IMP_RES_TAC (REWRITE_RULE [BAG_DELETE] BAG_IN_BAG_DELETE) THEN
-    ELIM_TAC THEN FULL_SIMP_TAC hol_ss [SUB_BAG_INSERT, FINITE_BAG_THM],
+    ELIM_TAC THEN FULL_SIMP_TAC std_ss [SUB_BAG_INSERT, FINITE_BAG_THM],
     ASM_MESON_TAC [NOT_IN_SUB_BAG_INSERT]
   ]);
-
 
 val _ = print "Developing theory of bag cardinality\n"
 
@@ -1274,15 +1103,15 @@ val BCARD_induct = prove(
   REWRITE_TAC [BAG_CARD_RELn, arithmeticTheory.ADD1] THEN MESON_TAC []);
 
 val strong_BCARD_induct =
-  (Q.SPEC `\b n. BAG_CARD_RELn b n /\ P b n` >-
-   SIMP_RULE hol_ss [BCARD_imps]) BCARD_induct
+  BCARD_induct |> Q.SPEC `\b n. BAG_CARD_RELn b n /\ P b n`
+               |> SIMP_RULE std_ss [BCARD_imps]
 
 val BCARD_R_cases = prove(
   Term`!b n. BAG_CARD_RELn b n ==>
              (b = EMPTY_BAG) /\ (n = 0) \/
              (?b0 e m. (b = BAG_INSERT e b0) /\
                        BAG_CARD_RELn b0 m /\ (n = m + 1))`,
-  HO_MATCH_MP_TAC BCARD_induct THEN SIMP_TAC hol_ss [] THEN
+  HO_MATCH_MP_TAC BCARD_induct THEN SIMP_TAC std_ss [] THEN
   REPEAT STRIP_TAC THEN ELIM_TAC THEN ASM_MESON_TAC [BCARD_imps]);
 
 val BCARD_rwts = prove(
@@ -1290,52 +1119,31 @@ val BCARD_rwts = prove(
              (b = EMPTY_BAG) /\ (n = 0) \/
              (?b0 e m. (b = BAG_INSERT e b0) /\ (n = m + 1) /\
                        BAG_CARD_RELn b0 m)`,
-  MESON_TAC [BCARD_R_cases, BCARD_imps]);
+  METIS_TAC [BCARD_R_cases, BCARD_imps]);
 
 val BCARD_BINSERT_indifferent = prove(
   Term`!b n. BAG_CARD_RELn b n ==>
              !b0 e. (b = BAG_INSERT e b0) ==>
                     BAG_CARD_RELn b0 (n - 1) /\ ~(n = 0)`,
-  HO_MATCH_MP_TAC strong_BCARD_induct THEN
-  SIMP_TAC hol_ss [BAG_INSERT_NOT_EMPTY] THEN REPEAT STRIP_TAC THEN
-  Q.ASM_CASES_TAC `e = e'` THENL [
-    ELIM_TAC THEN IMP_RES_TAC BAG_INSERT_ONE_ONE THEN ELIM_TAC THEN
-    ARWT,
-    ALL_TAC
-  ] THEN
-  Q.SUBGOAL_THEN `?b'. b = BAG_INSERT e' b'` STRIP_ASSUME_TAC
-  THENL [
-    SIMP_TAC hol_ss [GSYM BAG_DELETE] THEN
-    MATCH_MP_TAC BAG_IN_BAG_DELETE THEN
-    Q.SUBGOAL_THEN `BAG_IN e' (BAG_INSERT e b)`
-      (REWRITE_RULE [BAG_IN_BAG_INSERT] >- STRIP_ASSUME_TAC)
-    THENL [
-      ARWT THEN REWRITE_TAC [BAG_IN_BAG_INSERT],
-      ELIM_TAC THEN FULL_SIMP_TAC hol_ss []
-    ],
-    RES_TAC THEN ELIM_TAC THEN
-    RULE_ASSUM_TAC (ONCE_REWRITE_RULE [BAG_INSERT_commutes]) THEN
-    FULL_SIMP_TAC hol_ss [BAG_INSERT_ONE_ONE] THEN ELIM_TAC THEN
-    REPEAT_TCL STRIP_THM_THEN SUBST_ALL_TAC
-      (Q.SPEC `n` arithmeticTheory.num_CASES) THEN
-    FULL_SIMP_TAC hol_ss [arithmeticTheory.ADD1] THEN
-    ASM_MESON_TAC [BCARD_imps]
-  ]);
+  HO_MATCH_MP_TAC strong_BCARD_induct THEN SRW_TAC [][] THEN
+  FULL_SIMP_TAC (srw_ss()) [BAG_INSERT_EQUAL] THEN1 SRW_TAC [][] THEN
+  `BAG_CARD_RELn k (n - 1) /\ n <> 0` by METIS_TAC [] THEN
+  `n = (n - 1) + 1` by DECIDE_TAC THEN METIS_TAC [BCARD_imps]);
 
 val BCARD_BINSERT' =
-  SIMP_RULE hol_ss [RIGHT_IMP_FORALL_THM] BCARD_BINSERT_indifferent
+  SIMP_RULE bool_ss [GSYM RIGHT_FORALL_IMP_THM] BCARD_BINSERT_indifferent
 
 val BCARD_EMPTY = prove(
   Term`!n. BAG_CARD_RELn EMPTY_BAG n = (n = 0)`,
   ONCE_REWRITE_TAC [BCARD_rwts] THEN
-  SIMP_TAC hol_ss [BAG_INSERT_NOT_EMPTY]);
+  SIMP_TAC std_ss [BAG_INSERT_NOT_EMPTY]);
 
 val BCARD_BINSERT = prove(
   Term`!b e n. BAG_CARD_RELn (BAG_INSERT e b) n =
                (?m. (n = m + 1) /\ BAG_CARD_RELn b m)`,
-  REPEAT GEN_TAC THEN EQ_TAC THEN STRIP_TAC THEN ELIM_TAC THENL [
+  SRW_TAC [][EQ_IMP_THM] THENL [
     IMP_RES_TAC BCARD_BINSERT' THEN Q.EXISTS_TAC `n - 1` THEN
-    ASM_SIMP_TAC hol_ss [],
+    ASM_SIMP_TAC std_ss [],
     ASM_MESON_TAC [BCARD_imps]
   ]);
 
@@ -1346,9 +1154,9 @@ val BCARD_R_det = prove(
              !n'. BAG_CARD_RELn b n' ==> (n' = n)`,
   HO_MATCH_MP_TAC BCARD_induct THEN CONJ_TAC THENL [
     ONCE_REWRITE_TAC [BCARD_rwts] THEN
-    SIMP_TAC hol_ss [BAG_INSERT_NOT_EMPTY],
+    SIMP_TAC std_ss [BAG_INSERT_NOT_EMPTY],
     REPEAT STRIP_TAC THEN IMP_RES_TAC BCARD_BINSERT THEN RES_TAC THEN
-    ASM_SIMP_TAC hol_ss []
+    ASM_SIMP_TAC std_ss []
   ]);
 
 val FINITE_BAGS_BCARD = prove(
@@ -1358,13 +1166,14 @@ val FINITE_BAGS_BCARD = prove(
 val BAG_CARD = new_specification
   ("BAG_CARD",["BAG_CARD"],
    CONV_RULE SKOLEM_CONV (
-    SIMP_RULE hol_ss
+    SIMP_RULE std_ss
        [GSYM boolTheory.RIGHT_EXISTS_IMP_THM] FINITE_BAGS_BCARD));
 
 val BAG_CARD_EMPTY =
-  (Q.SPEC `EMPTY_BAG`  >- SIMP_RULE hol_ss [FINITE_EMPTY_BAG] >-
-   ONCE_REWRITE_RULE [BCARD_rwts] >-
-   SIMP_RULE hol_ss [BAG_INSERT_NOT_EMPTY]) BAG_CARD;
+  BAG_CARD |> Q.SPEC `EMPTY_BAG`
+           |> SIMP_RULE std_ss [FINITE_EMPTY_BAG]
+           |> ONCE_REWRITE_RULE [BCARD_rwts]
+           |> SIMP_RULE std_ss [BAG_INSERT_NOT_EMPTY]
 val _ = save_thm("BAG_CARD_EMPTY", BAG_CARD_EMPTY);
 val _ = export_rewrites ["BAG_CARD_EMPTY"];
 
@@ -1372,19 +1181,17 @@ val BCARD_0 = Q.store_thm(
   "BCARD_0",
   `!b. FINITE_BAG b ==> ((BAG_CARD b = 0) = (b = EMPTY_BAG))`,
   GEN_TAC THEN STRIP_TAC THEN EQ_TAC THEN
-  SIMP_TAC hol_ss [BAG_CARD_EMPTY] THEN
+  SIMP_TAC std_ss [BAG_CARD_EMPTY] THEN
   IMP_RES_TAC BAG_CARD THEN DISCH_THEN SUBST_ALL_TAC THEN
-  RULE_ASSUM_TAC (
-    ONCE_REWRITE_RULE [BCARD_rwts] >- SIMP_RULE hol_ss []) THEN
-  carwt);
+  FULL_SIMP_TAC (srw_ss()) [Once BCARD_rwts]);
 
 val BAG_CARD_EL_BAG = prove(
   Term`!e. BAG_CARD (EL_BAG e) = 1`,
-  GEN_TAC THEN SIMP_TAC hol_ss [EL_BAG] THEN
+  GEN_TAC THEN SIMP_TAC std_ss [EL_BAG] THEN
   Q.SUBGOAL_THEN `FINITE_BAG (BAG_INSERT e EMPTY_BAG)` ASSUME_TAC
   THENL [MESON_TAC [FINITE_BAG_INSERT, FINITE_EMPTY_BAG],
          ALL_TAC] THEN IMP_RES_TAC BAG_CARD THEN
-  FULL_SIMP_TAC hol_ss [BCARD_RWT])
+  FULL_SIMP_TAC std_ss [BCARD_RWT])
 
 val BAG_CARD_INSERT = prove(
   Term`!b. FINITE_BAG b ==>
@@ -1393,7 +1200,7 @@ val BAG_CARD_INSERT = prove(
   Q.SUBGOAL_THEN `FINITE_BAG (BAG_INSERT e b)` ASSUME_TAC THENL [
     ASM_MESON_TAC [FINITE_BAG_INSERT], ALL_TAC] THEN
   IMP_RES_TAC BAG_CARD THEN
-  FULL_SIMP_TAC hol_ss [BCARD_RWT] THEN IMP_RES_TAC BCARD_R_det);
+  FULL_SIMP_TAC std_ss [BCARD_RWT] THEN IMP_RES_TAC BCARD_R_det);
 
 val BAG_CARD_THM = save_thm(
   "BAG_CARD_THM",
@@ -1405,15 +1212,15 @@ val BCARD_SUC = Q.store_thm(
        !n. (BAG_CARD b = SUC n) =
            (?b0 e. (b = BAG_INSERT e b0) /\ (BAG_CARD b0 = n))`,
   GEN_TAC THEN STRUCT_CASES_TAC (Q.SPEC `b` BAG_cases) THEN
-  SIMP_TAC hol_ss [BAG_CARD_THM, BAG_INSERT_NOT_EMPTY,
+  SIMP_TAC std_ss [BAG_CARD_THM, BAG_INSERT_NOT_EMPTY,
                    FINITE_BAG_THM, arithmeticTheory.ADD1] THEN
   REPEAT STRIP_TAC THEN EQ_TAC THEN STRIP_TAC THENL [
     ASM_MESON_TAC [],
-    FIRST_ASSUM (Q.AP_TERM `BAG_CARD` >- MP_TAC) THEN
-    ASM_SIMP_TAC hol_ss [BAG_CARD_THM] THEN
+    FIRST_ASSUM (MP_TAC o Q.AP_TERM `BAG_CARD`) THEN
+    ASM_SIMP_TAC std_ss [BAG_CARD_THM] THEN
     Q.SUBGOAL_THEN `FINITE_BAG b0'` ASSUME_TAC THENL [
       ASM_MESON_TAC [FINITE_BAG_THM],
-      ASM_SIMP_TAC hol_ss [BAG_CARD_THM]
+      ASM_SIMP_TAC std_ss [BAG_CARD_THM]
     ]
   ]);
 
@@ -1421,11 +1228,11 @@ val BAG_CARD_BAG_INN = Q.store_thm(
   "BAG_CARD_BAG_INN",
   `!b. FINITE_BAG b ==> !n e. BAG_INN e n b ==> n <= BAG_CARD b`,
   HO_MATCH_MP_TAC STRONG_FINITE_BAG_INDUCT THEN
-  SIMP_TAC hol_ss [BAG_CARD_THM, BAG_INN_BAG_INSERT,
+  SIMP_TAC std_ss [BAG_CARD_THM, BAG_INN_BAG_INSERT,
                     BAG_INN_EMPTY_BAG] THEN REPEAT STRIP_TAC
   THENL [
-    ELIM_TAC THEN RES_TAC THEN ASM_SIMP_TAC hol_ss [],
-    RES_TAC THEN ASM_SIMP_TAC hol_ss []
+    ELIM_TAC THEN RES_TAC THEN ASM_SIMP_TAC std_ss [],
+    RES_TAC THEN ASM_SIMP_TAC std_ss []
   ]);
 
 (* --------------------------------------------------------------------
@@ -1805,7 +1612,7 @@ val COMMUTING_ITBAG_RECURSES = store_thm(
 val BAG_GEN_SUM_def =
  new_definition
  ("BAG_GEN_SUM_def",
-  ``BAG_GEN_SUM bag n = ITBAG (+) bag n``);
+  ``BAG_GEN_SUM bag (n:num) = ITBAG (+) bag n``);
 
 val BAG_GEN_PROD_def =
  new_definition
@@ -1829,7 +1636,7 @@ val BAG_GEN_SUM_TAILREC = store_thm
  GEN_TAC THEN STRIP_TAC THEN
  SIMP_TAC bool_ss [BAG_GEN_SUM_def] THEN
  HO_MATCH_MP_TAC (SPEC_ALL COMMUTING_ITBAG_INSERT) THEN
- RW_TAC hol_ss []);
+ RW_TAC std_ss []);
 
 val BAG_GEN_SUM_REC = store_thm
 ("BAG_GEN_SUM_REC",
@@ -1838,7 +1645,7 @@ val BAG_GEN_SUM_REC = store_thm
   GEN_TAC THEN REPEAT STRIP_TAC THEN
   SIMP_TAC bool_ss [BAG_GEN_SUM_def] THEN
   HO_MATCH_MP_TAC (SPEC_ALL COMMUTING_ITBAG_RECURSES) THEN
-  RW_TAC hol_ss []);
+  RW_TAC std_ss []);
 
 val BAG_GEN_PROD_TAILREC = store_thm
 ("BAG_GEN_PROD_TAILREC",
@@ -1847,7 +1654,7 @@ val BAG_GEN_PROD_TAILREC = store_thm
  GEN_TAC THEN STRIP_TAC THEN
  SIMP_TAC bool_ss [BAG_GEN_PROD_def] THEN
  HO_MATCH_MP_TAC (SPEC_ALL COMMUTING_ITBAG_INSERT) THEN
- RW_TAC hol_ss []);
+ RW_TAC std_ss []);
 
 val BAG_GEN_PROD_REC = store_thm
 ("BAG_GEN_PROD_REC",
@@ -1856,7 +1663,7 @@ val BAG_GEN_PROD_REC = store_thm
  GEN_TAC THEN REPEAT STRIP_TAC THEN
  SIMP_TAC bool_ss [BAG_GEN_PROD_def] THEN
  HO_MATCH_MP_TAC (SPEC_ALL COMMUTING_ITBAG_RECURSES) THEN
- RW_TAC hol_ss []);
+ RW_TAC std_ss []);
 
 val BAG_GEN_PROD_EQ_1 = Q.store_thm
 ("BAG_GEN_PROD_EQ_1",
@@ -1864,8 +1671,8 @@ val BAG_GEN_PROD_EQ_1 = Q.store_thm
  HO_MATCH_MP_TAC STRONG_FINITE_BAG_INDUCT THEN REPEAT STRIP_TAC THENL
  [METIS_TAC [BAG_GEN_PROD_EMPTY],
   Q.PAT_ASSUM `p=q` MP_TAC THEN
-  RW_TAC hol_ss [Once BAG_GEN_PROD_TAILREC] THEN
-  RES_TAC THEN FULL_SIMP_TAC hol_ss []]);
+  RW_TAC std_ss [Once BAG_GEN_PROD_TAILREC] THEN
+  RES_TAC THEN FULL_SIMP_TAC std_ss []]);
 
 val BAG_GEN_PROD_ALL_ONES = Q.store_thm
 ("BAG_GEN_PROD_ALL_ONES",
@@ -1873,8 +1680,8 @@ val BAG_GEN_PROD_ALL_ONES = Q.store_thm
  HO_MATCH_MP_TAC STRONG_FINITE_BAG_INDUCT THEN REPEAT STRIP_TAC THENL
  [METIS_TAC [NOT_IN_EMPTY_BAG],
   Q.PAT_ASSUM `p=q` MP_TAC THEN
-    RW_TAC hol_ss [BAG_GEN_PROD_TAILREC] THEN
-    `e=1` by METIS_TAC [BAG_GEN_PROD_EQ_1] THEN RW_TAC hol_ss [] THEN
+    RW_TAC std_ss [BAG_GEN_PROD_TAILREC] THEN
+    `e=1` by METIS_TAC [BAG_GEN_PROD_EQ_1] THEN RW_TAC std_ss [] THEN
     `!x. BAG_IN x b ==> (x = 1)` by METIS_TAC[] THEN
     METIS_TAC [BAG_IN_BAG_INSERT]]);
 
@@ -1883,7 +1690,7 @@ val BAG_GEN_PROD_POSITIVE = Q.store_thm
  `!b. FINITE_BAG b ==> (!x. BAG_IN x b ==> 0 < x) ==> 0 < BAG_GEN_PROD b 1`,
  HO_MATCH_MP_TAC STRONG_FINITE_BAG_INDUCT THEN REPEAT STRIP_TAC THENL
  [METIS_TAC [BAG_GEN_PROD_EMPTY,ARITH `0<1`],
-  RW_TAC hol_ss [BAG_GEN_PROD_REC] THEN
+  RW_TAC std_ss [BAG_GEN_PROD_REC] THEN
   `0 < e` by METIS_TAC [BAG_IN_BAG_INSERT] THEN
   `0 < BAG_GEN_PROD b 1` by METIS_TAC [BAG_IN_BAG_INSERT] THEN
  METIS_TAC [arithmeticTheory.LESS_MULT2]]);
@@ -1896,7 +1703,7 @@ val BAG_EVERY =
 val BAG_EVERY_THM = store_thm ("BAG_EVERY_THM",
 ``(!P. (BAG_EVERY P EMPTY_BAG)) /\
   (!P e b. (BAG_EVERY P (BAG_INSERT e b) = P e /\ BAG_EVERY P b))``,
-SIMP_TAC hol_ss [BAG_EVERY, BAG_IN_BAG_INSERT,
+SIMP_TAC std_ss [BAG_EVERY, BAG_IN_BAG_INSERT,
 		 DISJ_IMP_THM, FORALL_AND_THM,
 		 NOT_IN_EMPTY_BAG]);
 
@@ -1907,7 +1714,7 @@ val BAG_ALL_DISTINCT_THM = store_thm ("BAG_ALL_DISTINCT_THM",
 ``BAG_ALL_DISTINCT EMPTY_BAG /\
   (!e b. (BAG_ALL_DISTINCT (BAG_INSERT e b) =
          ~(BAG_IN e b) /\ BAG_ALL_DISTINCT b))``,
-SIMP_TAC hol_ss [BAG_ALL_DISTINCT, EMPTY_BAG,
+SIMP_TAC std_ss [BAG_ALL_DISTINCT, EMPTY_BAG,
 		 BAG_IN, BAG_INN, BAG_INSERT,
 		 COND_RAND, COND_RATOR,
 		 COND_EXPAND_IMP, FORALL_AND_THM] THEN
@@ -1921,7 +1728,7 @@ val BAG_ALL_DISTINCT_BAG_MERGE = store_thm (
   "BAG_ALL_DISTINCT_BAG_MERGE",
   ``!b1 b2. BAG_ALL_DISTINCT (BAG_MERGE b1 b2) =
         (BAG_ALL_DISTINCT b1 /\  BAG_ALL_DISTINCT b2)``,
-  SIMP_TAC hol_ss [BAG_ALL_DISTINCT, BAG_MERGE,
+  SIMP_TAC std_ss [BAG_ALL_DISTINCT, BAG_MERGE,
                    GSYM FORALL_AND_THM, COND_RAND, COND_RATOR,
 		   COND_EXPAND_IMP] THEN
   REPEAT STRIP_TAC THEN
@@ -1934,7 +1741,7 @@ val BAG_ALL_DISTINCT_BAG_UNION = store_thm (
         BAG_ALL_DISTINCT (BAG_UNION b1 b2) =
         (BAG_ALL_DISTINCT b1 /\ BAG_ALL_DISTINCT b2 /\
          BAG_DISJOINT b1 b2)``,
-  SIMP_TAC hol_ss [BAG_ALL_DISTINCT, BAG_UNION,
+  SIMP_TAC std_ss [BAG_ALL_DISTINCT, BAG_UNION,
 		   BAG_DISJOINT, DISJOINT_DEF, EXTENSION,
 		   NOT_IN_EMPTY, IN_INTER,
 		   IN_SET_OF_BAG, BAG_IN,
@@ -1948,7 +1755,7 @@ val BAG_ALL_DISTINCT_DIFF = store_thm (
   ``!b1 b2.
        BAG_ALL_DISTINCT b1 ==>
        BAG_ALL_DISTINCT (BAG_DIFF b1 b2)``,
-  SIMP_TAC hol_ss [BAG_ALL_DISTINCT, BAG_DIFF] THEN
+  SIMP_TAC std_ss [BAG_ALL_DISTINCT, BAG_DIFF] THEN
   REPEAT STRIP_TAC THEN
   `b1 e <= 1` by PROVE_TAC[] THEN
   bossLib.DECIDE_TAC);
@@ -1959,11 +1766,11 @@ val BAG_IN_BAG_DIFF_ALL_DISTINCT = store_thm (
   ``!b1 b2 e. BAG_ALL_DISTINCT b1 ==>
        (BAG_IN e (BAG_DIFF b1 b2) =
         BAG_IN e b1 /\ ~BAG_IN e b2)``,
-  SIMP_TAC hol_ss [BAG_ALL_DISTINCT,
+  SIMP_TAC std_ss [BAG_ALL_DISTINCT,
 		   BAG_IN, BAG_INN, BAG_DIFF] THEN
   REPEAT STRIP_TAC THEN
   `b1 e <= 1` by PROVE_TAC[] THEN
-  Cases_on `b1 e >= 1` THEN ASM_SIMP_TAC hol_ss []
+  Cases_on `b1 e >= 1` THEN ASM_SIMP_TAC std_ss []
 );
 
 val NOT_BAG_IN = Q.store_thm
@@ -2027,9 +1834,6 @@ val BAG_GEN_PROD_UNION = Q.store_thm
     Taken from Isabelle development of same.
    ---------------------------------------------------------------------- *)
 
-val _ = overload_on ("+", ``BAG_UNION``)
-val _ = overload_on ("-", ``BAG_DIFF``)
-
 (* The 1 is from the fact that is one step of the relation, other uses
    might want to take the transitive closure of this. *)
 val mlt1_def = new_definition(
@@ -2043,49 +1847,6 @@ val BAG_NOT_LESS_EMPTY = store_thm(
   ``~mlt1 r b {||}``,
   SRW_TAC [][mlt1_def]);
 val _ = export_rewrites ["BAG_NOT_LESS_EMPTY"]
-
-val add_eq_conv_diff = prove(
-  ``(M + {|a|} = N + {|b|}) =
-    (M = N) /\ (a = b) \/
-    (M = N - {|a|} + {|b|}) /\ (N = M - {|b|} + {|a|})``,
-  SRW_TAC [][BAG_UNION, BAG_DIFF, FUN_EQ_THM, BAG_INSERT, EMPTY_BAG] THEN
-  Cases_on `a = b` THEN SRW_TAC [][] THENL [
-    EQ_TAC THEN1 SRW_TAC [][] THEN STRIP_TAC THEN
-    Q.X_GEN_TAC `x` THEN
-    REPEAT (POP_ASSUM (Q.SPEC_THEN `x` MP_TAC)) THEN SRW_TAC [][] THEN
-    DECIDE_TAC,
-
-    EQ_TAC THEN STRIP_TAC THEN REPEAT CONJ_TAC THEN
-    Q.X_GEN_TAC `x` THEN
-    REPEAT (FIRST_X_ASSUM (Q.SPEC_THEN `x` MP_TAC)) THEN
-    SRW_TAC [][] THEN DECIDE_TAC
-  ]);
-
-
-val insert_diffM2 = prove(
-  ``BAG_IN x M ==> (M - {|x|} + {|x|} = M)``,
-  SRW_TAC [][BAG_UNION, BAG_DIFF, BAG_INSERT, EMPTY_BAG, FUN_EQ_THM, BAG_IN,
-             BAG_INN] THEN
-  SRW_TAC [][] THEN DECIDE_TAC);
-
-val add_eq_conv_ex = prove(
-  ``(M + {|a|} = N + {|b|}) =
-    (M = N) /\ (a = b) \/
-    ?k. (M = k + {|b|}) /\ (N = k + {|a|})``,
-  SRW_TAC [][add_eq_conv_diff] THEN Cases_on `a = b` THENL [
-    SRW_TAC [][EQ_IMP_THM] THEN
-    FULL_SIMP_TAC (srw_ss()) [insert_diffM2] THEN
-    POP_ASSUM ACCEPT_TAC,
-
-    SRW_TAC [][] THEN EQ_TAC THEN STRIP_TAC THENL [
-      POP_ASSUM SUBST_ALL_TAC THEN SRW_TAC [][] THEN
-      `BAG_IN b M` by METIS_TAC [BAG_IN_BAG_UNION, BAG_IN_BAG_INSERT] THEN
-      SRW_TAC [][insert_diffM2],
-
-      SRW_TAC [][]
-    ]
-  ]);
-
 
 val BAG_LESS_ADD = store_thm(
   "BAG_LESS_ADD",
